        % ------------------------------------------ %
        %                      (2.8)                 %
        % ------------------------------------------ %
        Given the matrix
        \[
            \bold{A} = \begin{bmatrix}
                1 & 2 \\
                2 & -2
            \end{bmatrix}
        \]
        find the eigenvalues $\lambda_1$ and $\lambda_2$ and the associated eigenvectors $\bold{e}_1$ and $\bold{e}_2$. Determine the spectral decomposition \textbf{(2-16)} of $\bold{A}$.
        \par
        \[
            0 = \left|\bold{A} - \lambda\bold{I}\right|
            =
            \left|
            \begin{matrix}
                1 - \lambda & 2 \\
                2 & -2 - \lambda
            \end{matrix}
            \right|
            =
            \left(1 - \lambda\right)\left(-2-\lambda\right) - 4
            =
            -2 + 2\lambda - \lambda + \lambda^2 - 4
            =
        \]
        \[
            = \lambda^2 + \lambda - 6
            = \left(\lambda + 3 \right)\left(\lambda - 2\right)
        \]
        The eigenvalues are -3 and 2.
        \newline
        $\underline{\lambda_1 = -3}$:
        \[
            \bold{A}\bold{x}_1 = \lambda\bold{x}_1
            \Rightarrow
            \bold{A} = \begin{bmatrix}
                1 & 2 \\
                2 & -2
            \end{bmatrix}
            \begin{bmatrix}
                x_1 \\
                x_2
            \end{bmatrix}
            =
            \begin{bmatrix}
                -3x_1 \\
                -3x_2
            \end{bmatrix}
        \]
        \[
            x_1 + 2x_2 = -3x_1
            \Rightarrow
            -4x_1 = 2x_2
            \Rightarrow
            -2x_1 = x_2
        \]
        and
        \[
            2x_1 - 2x_2 = -3x_1
            \Rightarrow
            2x_1 = -x_2
            \Rightarrow
            -2x_1 = x_2
        \]
        So $\bold{x}_1 = \begin{bmatrix}
            1 \\
            -2
        \end{bmatrix}$ and normalizing $\bold{e}_1 = \begin{bmatrix}
            1/\sqrt{5} \\
            -2/\sqrt{5}
        \end{bmatrix}$.
        \newline
        $\underline{\lambda_2 = 2}$:
        \[
            \bold{A}\bold{x}_2 = \lambda\bold{x}_2
            \Rightarrow
            \bold{A} = \begin{bmatrix}
                1 & 2 \\
                2 & -2
            \end{bmatrix}
            \begin{bmatrix}
                x_1 \\
                x_2
            \end{bmatrix}
            =
            \begin{bmatrix}
                2x_1 \\
                2x_2
            \end{bmatrix}
        \]
        \[
            x_1 + 2x_2 = 2x_1
            \Rightarrow
            2x_2 = x_1
        \]
        and
        \[
            2x_1 - 2x_2 = 2x_1
            \Rightarrow
            x_2 = 4x_1
            \Rightarrow
            x_1 = 2x_2
        \]
        So $\bold{x}_2 = \begin{bmatrix}
            2 \\
            1
        \end{bmatrix}$ and normalizing $\bold{e}_2 = \begin{bmatrix}
            2/\sqrt{5} \\
            1/\sqrt{5}
        \end{bmatrix}$.
        \newline
        \[
            \bold{A} = \sum_{k=1}^2{\lambda_k \bold{e}_k \bold{e}_k^\prime}
            =
            -3 \begin{bmatrix}
                1/\sqrt{5} \\
                -2/\sqrt{5}
            \end{bmatrix}
            \begin{bmatrix}
                1/\sqrt{5} & -2/\sqrt{5}
            \end{bmatrix}
            +
            2 \begin{bmatrix}
                2/\sqrt{5} \\
                1/\sqrt{5}
            \end{bmatrix}
            \begin{bmatrix}
                2/\sqrt{5} & 1/\sqrt{5}
            \end{bmatrix}
            =
        \]
        \[
            =
            \frac{1}{5}
            \left(
                -3
                \begin{bmatrix}
                    1 & -2 \\
                    2 & 4
                \end{bmatrix}
                +
                2
                \begin{bmatrix}
                    4 & 2 \\
                    2 & 1
                \end{bmatrix}
            \right)
            =
            \frac{1}{5}
            \left(
                -
                \begin{bmatrix}
                    3 & -6 \\
                    -6 & 12
                \end{bmatrix}
                +
                \begin{bmatrix}
                    8 & 4 \\
                    4 & 2
                \end{bmatrix}
            \right)
            =
        \]
        \[
            \frac{1}{5}
            \begin{bmatrix}
                5 & 10 \\
                10 & -10
            \end{bmatrix}
            =
            \begin{bmatrix}
                1 & 2 \\
                2 & -2
            \end{bmatrix}
        \]