        % ------------------------------------------ %
        %                      (2.20)                %
        % ------------------------------------------ %
        Determine the square-root matrix $\bold{A}^{1/2}$, using the matrix $\bold{A}$ in \textbf{Exercise 2.3}. Also, determine
        $\bold{A}^{-1/2}$, and show that $\bold{A}^{1/2}\bold{A}^{-1/2} = \bold{A}^{-1/2}\bold{A}^{1/2} = \bold{I}$.
        \par
        \[
            \bold{A}
            =
            \begin{bmatrix}
                2 & 1 \\
                1 & 3
            \end{bmatrix}
        \]
        \[
            0 = \left|\bold{A} - \lambda\bold{I}\right|
            =
            \left|
            \begin{matrix}
                2 - \lambda & 1 \\
                1 & 3 - \lambda
            \end{matrix}
            \right|
            =
            \left(2 - \lambda\right)\left(3 - \lambda\right) - 1
            =
            \lambda^2 - 5\lambda + 6 - 1
            =
        \]
        \[
            =
            \left(\lambda - \frac{5 - \sqrt{5}}{2}\right)\left(\lambda - \frac{5 + \sqrt{5}}{2}\right)
        \]
        The eigenvalues are $\left\{\lambda_1, \lambda_2\right\} = \left\{\frac{5 - \sqrt{5}}{2}, \frac{5 + \sqrt{5}}{2}\right\}$.
        \newline
        To sumplify things, define variables $a$ and $b$,
        \[
            a = {(5-\sqrt(5))}^{1/2}
        \]
        \[
            b = {(5+\sqrt(5))}^{1/2}
        \]
        Using a few useful facts,
        \[
            a^{1/2}(1 + 5^{1/2}) = 2b^{1/2}
        \]
        and
        \[
            b^{1/2}(1 - 5^{1/2}) = -2a^{1/2}
        \]
        \underline{$\lambda_1 = \frac{5 - \sqrt{5}}{2}$:}
        \[
            \bold{A}\bold{x}_1 = \lambda_1 \bold{x}_1
            \Rightarrow
            \begin{bmatrix}
                2 & 1 \\
                1 & 3
            \end{bmatrix}
            \begin{bmatrix}
                x_1 \\
                x_2
            \end{bmatrix}
            =
            \begin{bmatrix}
                \left(\frac{5 - \sqrt{5}}{2}\right)x_1 \\
                \left(\frac{5 - \sqrt{5}}{2}\right)x_2
            \end{bmatrix}
        \]
        \[
            \Rightarrow
            \begin{bmatrix}
                \left(\frac{-1 + \sqrt{5}}{2}\right) & 1 \\
                1 & \left(\frac{1 + \sqrt{5}}{2}\right)
            \end{bmatrix}
            \begin{bmatrix}
                x_1 \\
                x_2
            \end{bmatrix}
            =
            \begin{bmatrix}
                0 \\
                0
            \end{bmatrix}
        \]
        \[
            \begin{bmatrix}
                \left(\frac{-1 + \sqrt{5}}{2}\right) & 1 \\
                1 & \left(\frac{1 + \sqrt{5}}{2}\right)
            \end{bmatrix}
            \overset{\text{Row 2} - \left(\frac{2}{\sqrt{5} - 1}\right)\text{Row 1}}{\longrightarrow}
            \begin{bmatrix}
                \left(\frac{-1 + \sqrt{5}}{2}\right) & 1 \\
                0 & 0
            \end{bmatrix}
        \]
        So $\left(\frac{-1 + 5^{1/2}}{2}\right)x_1 + x_2 = 0 \Rightarrow x_2 
        = -\left(\frac{-1 + 5^{1/2}}{2}\right)x_1 = \left(\frac{1 - 5^{1/2}}{2}\right)x_1$
        \newline
        We have $x_2 = \left(\frac{1 - 5^{1/2}}{2}\right)x_1$, so when $x = -1$, $x_2 = -\left(\frac{1 - 5^{1/2}}{2}\right) > 0$.
        \[
            {\left\|\bold{x}_1\right\|} = \frac{{\left(5 - 5^{1/2}\right)^{1/2}}}{2^{1/2}} = \frac{a^{1/2}}{2^{1/2}}
        \]
        \[
            \bold{x}_1
            =
            \begin{bmatrix}
                -1 \\
                -\left(\frac{1 - 5^{1/2}}{2}\right)
            \end{bmatrix}
            \Rightarrow
            \bold{e}_1
            =
            \frac{\bold{x}_1}{\left\|\bold{x}_1\right\|}
            =
            \frac{2^{1/2}}{a^{1/2}}
            \begin{bmatrix}
                -1 \\
                -\left(\frac{1 - 5^{1/2}}{2}\right)
            \end{bmatrix}
            =
            \begin{bmatrix}
                -\frac{2^{1/2}}{a^{1/2}} \\
                -\left(\frac{1 - 5^{1/2}}{2^{1/2}a^{1/2}}\right)\left(\frac{1 + 5^{1/2}}{1 + 5^{1/2}}\right)
            \end{bmatrix}
            =
            \begin{bmatrix}
                -{\left(2/a\right)}^{1/2} \\
                {\left(2/b\right)}^{1/2}
            \end{bmatrix}
        \]
        \newline
        \underline{$\lambda_2 = \frac{5 + \sqrt{5}}{2}$:}
        \[
            \bold{A}\bold{x}_2 = \lambda_2 \bold{x}_2
            \Rightarrow
            \begin{bmatrix}
                2 & 1 \\
                1 & 3
            \end{bmatrix}
            \begin{bmatrix}
                x_1 \\
                x_2
            \end{bmatrix}
            =
            \begin{bmatrix}
                \left(\frac{5 + \sqrt{5}}{2}\right)x_1 \\
                \left(\frac{5 + \sqrt{5}}{2}\right)x_2
            \end{bmatrix}
        \]
        \[
            =
            \begin{bmatrix}
                \left(\frac{-1 - \sqrt{5}}{2}\right) & 1 \\
                1 & \left(\frac{1 - \sqrt{5}}{2}\right)
            \end{bmatrix}
            \begin{bmatrix}
                x_1 \\
                x_2
            \end{bmatrix}
            =
            \begin{bmatrix}
                0 \\
                0
            \end{bmatrix}
        \]
        \[
            \begin{bmatrix}
                \left(\frac{-1 - \sqrt{5}}{2}\right) & 1 \\
                1 & \left(\frac{1 - \sqrt{5}}{2}\right)
            \end{bmatrix}
            \overset{\text{Row 2} + \left(\frac{2}{1 + \sqrt{5}}\right)\text{Row 1}}{\longrightarrow}
            \begin{bmatrix}
                \left(\frac{-1 - \sqrt{5}}{2}\right) & 1 \\
                0 & 0
            \end{bmatrix}
        \]
        So $\left(\frac{-1 - \sqrt{5}}{2}\right)x_1 + x_2 = 0 \Rightarrow x_2 = \left(\frac{1 + \sqrt{5}}{2}\right)x_1$
        \newline
        We have $x_2 = \left(\frac{1 + 5^{1/2}}{2}\right)x_1$, so when $x = 1$, $x_2 = \left(\frac{1 + 5^{1/2}}{2}\right) > 0$.
        \[
            {\left\|\bold{x}_2\right\|} = \frac{{\left(5 + 5^{1/2}\right)}^{1/2}}{2^{1/2}} = \frac{b^{1/2}}{2^{1/2}}
        \]
        \[
            \bold{x}_2
            =
            \begin{bmatrix}
                1 \\
                \left(\frac{1 + 5^{1/2}}{2}\right)
            \end{bmatrix}
            \Rightarrow
            \bold{e}_1
            =
            \frac{\bold{x}_2}{\left\|\bold{x}_2\right\|}
            =
            \frac{2^{1/2}}{b^{1/2}}
            \begin{bmatrix}
                1 \\
                \left(\frac{1 + 5^{1/2}}{2}\right)
            \end{bmatrix}
            =
            \begin{bmatrix}
                \frac{2^{1/2}}{b^{1/2}} \\
                \left(\frac{1 + 5^{1/2}}{2^{1/2}b^{1/2}}\right) \left(\frac{1 - 5^{1/2}}{1 - 5^{1/2}}\right)
            \end{bmatrix}
            =
            \begin{bmatrix}
                {\left(2/b\right)}^{1/2} \\
                {\left(2/a\right)}^{1/2}
            \end{bmatrix}
        \]
        We finally have all of the eigenvalues and eigenvectors,
        \[
            \bold{\Lambda} 
            =
            \begin{bmatrix}
                \lambda_1 & 0 \\
                0 & \lambda_2
            \end{bmatrix}
            =
            \begin{bmatrix}
                a/2 & 0 \\
                0 & b/2
            \end{bmatrix}
        \]
        \[
            \bold{P}
            =
            \begin{bmatrix}
                \bold{e}_1 & \bold{e}_2
            \end{bmatrix}
            =
            \begin{bmatrix}
                {\left(2/a\right)}^{1/2} & {\left(2/b\right)}^{1/2} \\
                -{\left(2/b\right)}^{1/2} & {\left(2/a\right)}^{1/2}
            \end{bmatrix}
        \]
        Now to find $\bold{A}^{1/2}$. Rewrite a few things,
        
        \[
            \bold{A}^{1/2}
            =
            2^{1/2}
            \begin{bmatrix}
                {\left(b/a^2\right)}^{1/2} & {\left(a/b^2\right)}^{1/2} \\
                {\left(a/b^2\right)}^{1/2} & {\left(2^2/a\right)}^{1/2}
            \end{bmatrix}
        \]