        % ------------------------------------------ %
        %                      (2.14)                %
        % ------------------------------------------ %
        Show that $\underset{\left(p \times p\right)}{\bold{Q}^\prime} \underset{\left(p \times p\right)}{\bold{A}} \underset{\left(p \times p\right)}{\bold{Q}}$ and $\underset{p \times p}{\bold{A}}$ have the same eigenvalues if $\bold{Q}$ is orthogonal.
        \newline
        \textit{Hint:} Let $\lambda$ be an eigenvalue of $\bold{A}$. Then $0 = \left|\bold{A} - \lambda \bold{I}\right|$. By \textbf{Exercise 2.13} and \textbf{Result 2A.11(e)}, we can write $0 = \left|\bold{Q}^\prime\right|\left|\bold{A} - \lambda \bold{I}\right| \left|\bold{Q}\right| = \left|\bold{Q}^\prime \bold{A} \bold{Q} - \lambda\bold{I}\right|$, since $\bold{Q}^\prime \bold{Q} = \bold{I}$ from \textbf{Exercise 2.11}.
        \par
        Answer is pretty much in the hint. We already know $\left|\bold{Q}^\prime\bold{Q}\right|$ = $\left|\bold{I}\right| = 1$. We also already know $\left|\bold{Q}^\prime\bold{Q}\right| = \left|\bold{Q}^\prime\right|\left|\bold{Q}\right|$ from \textbf{Result 2A.11(e)}. Not mentioned in the book, but the determinant is a scalar output, so it's also commutative, so $\left|\bold{Q}^\prime\bold{Q}\right| = \left|\bold{Q}^\prime\right|\left|\bold{Q}\right| = \left|\bold{Q}\right|\left|\bold{Q}^\prime\right|$.
        \[
            0
            =
            \left|\bold{A} - \lambda \bold{I}\right|
            =
            \left|\bold{Q}^\prime\bold{Q}\right|
            \left|\bold{A} - \lambda \bold{I}\right|
            =
            \left|\bold{Q}^\prime\right|
            \left|\bold{Q}\right|
            \left|\bold{A} - \lambda \bold{I}\right|
            =
            \left|\bold{Q}^\prime\right|
            \left|\bold{A} - \lambda \bold{I}\right|
            \left|\bold{Q}\right|
            =
        \]
        \[
            =
            \left|\bold{Q}^\prime\bold{A}\bold{Q} - \lambda \bold{Q}^\prime\bold{I}\bold{Q}\right|
            =
            \left|\bold{Q}^\prime\bold{A}\bold{Q} - \lambda \bold{Q}^\prime\bold{Q}\right|
            =
            \left|\bold{Q}^\prime\bold{A}\bold{Q} - \lambda \bold{I}\right|
        \]
        There it is, $0 = \left|\bold{A} - \lambda \bold{I}\right| = \left|\bold{Q}^\prime\bold{A}\bold{Q} - \lambda \bold{I}\right|$, so the eigenvalues of $\bold{A}$ are the same as those for $\bold{Q}^\prime\bold{A}\bold{Q}$.