        % ------------------------------------------ %
        %                      (2.3)                 %
        % ------------------------------------------ %
        Verify the following properties of transpose when
        \[
            \bold{A} = \begin{bmatrix}
                2 & 1 \\
                1 & 3
            \end{bmatrix}\text{,}\hspace{0.2in}
            \bold{B} = \begin{bmatrix}
                1 & 4 & 2 \\
                5 & 0 & 3
            \end{bmatrix}\text{,}\hspace{0.2in}\text{and}\hspace{0.2in}
            \bold{C} = \begin{bmatrix}
                1 & 4 \\
                3 & 2
            \end{bmatrix},
        \]
        \begin{enumerate}[label=(\alph*)]
            \item ${\left(\bold{A}^\prime\right)}^\prime = \bold{A}$
            

            \[
                {\left(\bold{A}^\prime\right)}^\prime = 
                {\left(
                    \begin{bmatrix}
                        2 & 1 \\
                        1 & 3
                    \end{bmatrix}^\prime
                    \right)}^\prime =
                {\left(
                    \begin{bmatrix}
                        2 & 1 \\
                        1 & 3
                    \end{bmatrix}
                    \right)}^\prime = 
                    \begin{bmatrix}
                        2 & 1 \\
                        1 & 3
                    \end{bmatrix} =
                    \bold{A}
            \]

            Matrix $\bold{A}$ is symmetric since $\bold{A} = \bold{A}^\prime$.


            \item ${\left(\bold{C}^\prime\right)}^{-1} = {\left(\bold{C}^{-1}\right)}^\prime$
            

            \[
                {\left(\bold{C}^\prime\right)}^{-1} = 
                {\left(
                    {\begin{bmatrix}
                        1 & 4 \\
                        3 & 2
                    \end{bmatrix}}^\prime\right)
                }^{-1} =
                {\begin{bmatrix}
                        1 & 3 \\
                        4 & 2
                \end{bmatrix}}^{-1} =
                \frac{1}{2-12}
                \begin{bmatrix}
                    2 & -3 \\
                    -4 & 1
                \end{bmatrix} =
                \begin{bmatrix}
                    -2/10 & 3/10 \\
                    4/10 & -1/10
                \end{bmatrix}
            \]

            \[
                {\left(\bold{C}^{-1}\right)}^\prime =
                {\left(
                    {\begin{bmatrix}
                        1 & 4 \\
                        3 & 2
                    \end{bmatrix}}^{-1}\right)
                }^\prime =
                {\frac{1}{2-12}
                {\begin{bmatrix}
                    2 & -4 \\
                    -3 & 1
                \end{bmatrix}}
                }^\prime =
                \begin{bmatrix}
                    -2/10 & 3/10 \\
                    4/10 & -1/10
                \end{bmatrix}
            \]
            So ${\left(\bold{C}^\prime\right)}^{-1} = {\left(\bold{C}^{-1}\right)}^\prime$.

            \item ${\left(\bold{AB}\right)}^\prime = \bold{B}^\prime \bold{A}^\prime$
            
            \[
                {\left(\bold{AB}\right)}^\prime = 
                {\left(
                    \begin{bmatrix}
                        2 & 1 \\
                        1 & 3
                    \end{bmatrix}
                    \begin{bmatrix}
                        1 & 4 & 2 \\
                        5 & 0 & 3
                    \end{bmatrix}
                \right)}^\prime =
                {\begin{bmatrix}
                    7 & 8 & 7 \\
                    16 & 4 & 11
                \end{bmatrix}}^\prime =
                \begin{bmatrix}
                    7 & 16 \\
                    8 & 4 \\
                    7 & 11
                \end{bmatrix}
            \]

            \[
                \bold{B}^\prime \bold{A}^\prime =
                {\begin{bmatrix}
                    1 & 4 & 2 \\
                    5 & 0 & 3
                \end{bmatrix}}^\prime
                {\begin{bmatrix}
                    2 & 1 \\
                    1 & 3
                \end{bmatrix}}^\prime =
                \begin{bmatrix}
                    1 & 5 \\
                    4 & 0 \\
                    2 & 3
                \end{bmatrix}
                \begin{bmatrix}
                    2 & 1 \\
                    1 & 3
                \end{bmatrix} =
                \begin{bmatrix}
                    7 & 16 \\
                    8 & 4 \\
                    7 & 11
                \end{bmatrix}
            \]

            So ${\left(\bold{AB}\right)}^\prime = \bold{B}^\prime \bold{A}^\prime$.

            \item For general $\underset{\left(m\times k\right)}{\bold{A}}$ and $\underset{\left(k\times l\right)}{\bold{B}}$, ${\left(\bold{AB}\right)}^\prime = \bold{B}^\prime\bold{A}^\prime$.
            
            \[
                {\left(\bold{AB}\right)}^\prime =
                {\left(
                \begin{bmatrix}
                    a_{11} & \dots & a_{1k} \\
                    \vdots & \ddots & \vdots \\
                    a_{m1} & \dots & a_{mk}
                \end{bmatrix}
                \begin{bmatrix}
                    b_{11} & \dots & b_{1\ell} \\
                    \vdots & \ddots & \vdots \\
                    b_{k1} & \dots & b_{k\ell}
                \end{bmatrix}
                \right)}^\prime = 
                {\left(
                \begin{bmatrix}
                    \sum_{i=1}^k{a_{1i}b_{i1}} & \dots & \sum_{i=1}^k{a_{1i}b_{i\ell}} \\
                    \vdots & \ddots & \vdots \\
                    \sum_{i=1}^k{a_{mi}b_{i1}} & \dots & \sum_{i=1}^k{a_{mi}b_{i\ell}}
                \end{bmatrix}
                \right)}^\prime = 
            \]
            \[
                = \begin{bmatrix}
                    \sum_{i=1}^k{a_{1i}b_{i1}} & \dots & \sum_{i=1}^k{a_{mi}b_{i1}} \\
                    \vdots & \ddots & \vdots \\
                    \sum_{i=1}^k{a_{1i}b_{i\ell}} & \dots & \sum_{i=1}^k{a_{mi}b_{i\ell}}
                \end{bmatrix}
            \]

            \[
                \bold{B}^\prime \bold{A}^\prime = 
                \begin{bmatrix}
                    b_{11} & \dots & b_{1\ell} \\
                    \vdots & \ddots & \vdots \\
                    b_{k1} & \dots & b_{k\ell}
                \end{bmatrix}^\prime
                \begin{bmatrix}
                    a_{11} & \dots & a_{1k} \\
                    \vdots & \ddots & \vdots \\
                    a_{m1} & \dots & a_{mk}
                \end{bmatrix}^\prime =
                \begin{bmatrix}
                    b_{11} & \dots & b_{k1} \\
                    \vdots & \ddots & \vdots \\
                    b_{1\ell} & \dots & b_{k\ell}
                \end{bmatrix}
                \begin{bmatrix}
                    a_{11} & \dots & a_{m1} \\
                    \vdots & \ddots & \vdots \\
                    a_{1k} & \dots & a_{mk}
                \end{bmatrix} =
            \]

            \[
                = \begin{bmatrix}
                    \sum_{i=1}^k{b_{i1}a_{1i}} & \dots & \sum_{i=1}^k{b_{i1}a_{mi}} \\
                    \vdots & \ddots & \vdots \\
                    \sum_{i=1}^k{b_{i\ell}a_{1i}} & \dots & \sum_{i=1}^k{b_{i\ell}a_{mi}}
                \end{bmatrix} = \begin{bmatrix}
                    \sum_{i=1}^k{a_{1i}b_{i1}} & \dots & \sum_{i=1}^k{a_{mi}b_{i1}} \\
                    \vdots & \ddots & \vdots \\
                    \sum_{i=1}^k{a_{1i}b_{i\ell}} & \dots & \sum_{i=1}^k{a_{mi}b_{i\ell}}
                \end{bmatrix}
            \]
        \end{enumerate}
        So ${\left(\bold{AB}\right)}^\prime = \bold{B}^\prime\bold{A}^\prime$.