Repeat Exercise 3.14 using the data matrix
\[
    \begin{bNiceArray}{ccc}
        1 & 4 & 3 \\
        6 & 2 & 6 \\
        8 & 3 & 3
    \end{bNiceArray}
\]
and the linear combinations
\[
    \textbf{b}^{\prime}\textbf{X}
    =
    \begin{bNiceArray}{ccc}
        1 & 1 & 1
    \end{bNiceArray}
    \begin{bNiceArray}{c}
        X_1 \\
        X_2 \\
        X_3
    \end{bNiceArray}
\]
\[
    \textbf{c}^{\prime}\textbf{X}
    =
    \begin{bNiceArray}{ccc}
        1 & 2 & -3
    \end{bNiceArray}
    \begin{bNiceArray}{c}
        X_1 \\
        X_2 \\
        X_3
    \end{bNiceArray}
\]
\begin{enumerate}[label=(\alph*)]
    \item Evaluate the sample means, variances, and covariance of $\textbf{b}^{\prime}\textbf{X}$ and $\textbf{c}^{\prime}\textbf{X}$ from first principles. That is, calculate the observed values of $\textbf{b}^{\prime}\textbf{X}$ and $\textbf{c}^{\prime}\textbf{X}$ and then use the sample mean, variance, and covariance formulas.
    \[
        \begin{NiceArray}{l}
            \textbf{b}^{\prime}\textbf{x}_1 = 1x_{11} + 1x_{12} + 1x_{13} = 1(1) + 1(4) + 1(3) = 8 \\
            \textbf{b}^{\prime}\textbf{x}_2 = 1x_{21} + 1x_{22} + 1x_{23} = 1(6) + 1(2) + 1(6) = 14 \\
            \textbf{b}^{\prime}\textbf{x}_3 = 1x_{31} + 1x_{32} + 1x_{33} = 1(8) + 1(3) + 1(3) = 14 \\
        \end{NiceArray}
    \]
    \[
        \text{Sample mean}
        =
        \frac{(8 + 14 + 14)}{3}
        =
        12
    \]
    \[
        \text{Sample variance}
        =
        \frac{{(8 - 12)}^2
        +
        {(14 - 12)}^2
        +
        {(14 - 12)}^2
        }{3 - 1}
        =
        12
    \]
    \[
        \begin{NiceArray}{l}
            \textbf{c}^{\prime}\textbf{x}_1 = 1x_{11} + 2x_{12} - 3x_{13} = 1(1) + 2(4) - 3(3) = 0 \\
            \textbf{c}^{\prime}\textbf{x}_2 = 1x_{21} + 2x_{22} - 3x_{23} = 1(6) + 2(2) - 3(6) = -8 \\
            \textbf{c}^{\prime}\textbf{x}_3 = 1x_{31} + 2x_{32} - 3x_{33} = 1(8) + 2(3) - 3(3) = 5 \\
        \end{NiceArray}
    \]
    \[
        \text{Sample mean}
        =
        \frac{(0 - 8 + 5)}{3}
        =
        -1
    \]
    \[
        \text{Sample variance}
        =
        \frac{{(0 + 1)}^2
        +
        {(-8 + 1)}^2
        +
        {(5 + 1)}^2
        }{3 - 1}
        =
        43
    \]
    The covariance between $\textbf{b}^{\prime}\textbf{X}$ and $\textbf{c}^{\prime}\textbf{X}$
    \[
        \text{Sample covariance}
        =
    \]
    \[
        =
        \frac{(8 - 12)(0 + 1)
        +
        (14 - 12)(-8 + 1)
        +
        (14 - 12)(5 + 1)
        }{3 - 1}
        =
    \]
    \[
        =
        -3
    \]
    \item Calculate the sample means, variances, covariance of $\textbf{B}^{\prime}\textbf{X}$ and $\textbf{c}^{\prime}\textbf{X}$ using (3-36). 
    Compare the results in (a) and (b).
    \newline
    \par
    First, compute $\bar{\textbf{x}}$ and $\textbf{S}_{\textbf{X}}$
    \[
        \bar{\textbf{x}}
        =
        \frac{1}{n} \textbf{X}^{\prime} \textbf{1}_n
        =
        \frac{1}{3} \textbf{X}^{\prime} \textbf{1}_3
        =
        \frac{1}{3}
        \begin{bNiceArray}{ccc}
            1 & 6 & 8 \\
            4 & 2 & 3 \\
            3 & 6 & 3
        \end{bNiceArray}
        \begin{bNiceArray}{c}
            1 \\
            1 \\
            1
        \end{bNiceArray}
        =
        \frac{1}{3}
        \begin{bNiceArray}{c}
            15 \\
            9 \\
            12
        \end{bNiceArray}
        =
        \begin{bNiceArray}{c}
            5 \\
            3 \\
            4
        \end{bNiceArray}
    \]
    The deviance is
    \[
        \textbf{X} - \textbf{1}_n \bar{\textbf{x}}^{\prime}
        =
        \textbf{X} - \textbf{1}_3 \bar{\textbf{x}}^{\prime}
        =
        \begin{bNiceArray}{ccc}
            1 & 4 & 3 \\
            6 & 2 & 6 \\
            8 & 3 & 3
        \end{bNiceArray}
        -
        \begin{bNiceArray}{cc}
            1 \\
            1 \\
            1
        \end{bNiceArray}
        \begin{bNiceArray}{ccc}
            5 & 3 & 4 \\
        \end{bNiceArray}
        =
    \]
    \[
        =
        \begin{bNiceArray}{ccc}
            1 & 4 & 3 \\
            6 & 2 & 6 \\
            8 & 3 & 3
        \end{bNiceArray}
        -
        \begin{bNiceArray}{ccc}
            5 & 3 & 4 \\
            5 & 3 & 4 \\
            5 & 3 & 4
        \end{bNiceArray}
        =
        \begin{bNiceArray}{rrr}
            -4 & 1 & -1 \\
            1 & -1 & 2 \\
            3 & 0 & -1
        \end{bNiceArray}
    \]
    Using the deviance to get $\textbf{S}_{\textbf{X}}$
    \[
        \textbf{S}_{\textbf{X}}
        =
        \left(\frac{1}{n - 1}\right)
        {\left(\textbf{X} - \textbf{1}_n \bar{\textbf{x}}^{\prime}\right)}^{\prime}
        \left(\textbf{X} - \textbf{1}_n \bar{\textbf{x}}^{\prime}\right)
        =
    \]
    \[
        =
        \left(\frac{1}{3 - 1}\right)
        \begin{bNiceArray}{rrr}
            -4 & 1 & 3 \\
            1 & -1 & 0 \\
            -1 & 2 & -1
        \end{bNiceArray}
        \begin{bNiceArray}{rrr}
            -4 & 1 & -1 \\
            1 & -1 & 2 \\
            3 & 0 & -1
        \end{bNiceArray}
        =
    \]
    \[
        =
        \left(\frac{1}{3 - 1}\right)
        \begin{bNiceArray}{rrr}
            26 & -5 & 3 \\
            -5 & 2 & -3 \\
            3 & -3 & 6
        \end{bNiceArray}
        =
        \begin{bNiceArray}{rrr}
            13 & -5/2 & 3/2 \\
            -5/2 & 1 & -3/2 \\
            3/2 & -3/2 & 3
        \end{bNiceArray}
    \]
    \[
        \text{sample mean}
        =
        E[\textbf{b}^{\prime}\textbf{X}]
        =
        \textbf{b}^{\prime} E[\textbf{X}]
        =
        \textbf{b}^{\prime} \bar{\textbf{x}}
        =
        \begin{bNiceArray}{rrr}
            1 & 1 & 1
        \end{bNiceArray}
        \begin{bNiceArray}{c}
            5 \\
            3 \\
            4
        \end{bNiceArray}
        =
        5 + 3 + 4
        =
        12
    \]
    \[
        \text{sample variance}
        =
        V[\textbf{b}^{\prime}\textbf{X}]
        =
        \textbf{b}^{\prime} V[\textbf{X}]\textbf{c}
        =
        \textbf{b}^{\prime} \textbf{S}_{\textbf{X}} \textbf{c}
        =
    \]
    \[
        =
        \begin{bNiceArray}{rrr}
            1 & 1 & 1
        \end{bNiceArray}
        \begin{bNiceArray}{rrr}
            13 & -5/2 & 3/2 \\
            -5/2 & 1 & -3/2 \\
            3/2 & -3/2 & 3
        \end{bNiceArray}
        \begin{bNiceArray}{r}
            1 \\
            1 \\
            1
        \end{bNiceArray}
        =
        \begin{bNiceArray}{rrr}
            12 & -3 & 3
        \end{bNiceArray}
        \begin{bNiceArray}{r}
            1 \\
            1 \\
            1
        \end{bNiceArray}
        =
        12
    \]
    \[
        \text{sample mean}
        =
        E[\textbf{c}^{\prime}\textbf{X}]
        =
        \textbf{c}^{\prime} E[\textbf{X}]
        =
        \textbf{c}^{\prime} \bar{\textbf{x}}
        =
        \begin{bNiceArray}{rrr}
            1 & 2 & -3
        \end{bNiceArray}
        \begin{bNiceArray}{c}
            5 \\
            3 \\
            4
        \end{bNiceArray}
        =
    \]
    \[
        =
        5 + 6 -12
        =
        -1
    \]
    \[
        \text{sample variance}
        =
        V[\textbf{c}^{\prime}\textbf{X}]
        =
        \textbf{c}^{\prime} V[\textbf{X}] \textbf{c}
        =
        \textbf{c}^{\prime} \textbf{S}_{\textbf{X}} \textbf{c}
        =
    \]
    \[
        =
        \begin{bNiceArray}{rrr}
            1 & 2 & -3
        \end{bNiceArray}
        \begin{bNiceArray}{rrr}
            13 & -5/2 & 3/2 \\
            -5/2 & 1 & -3/2 \\
            3/2 & -3/2 & 3
        \end{bNiceArray}
        \begin{bNiceArray}{r}
            1 \\
            2 \\
            -3
        \end{bNiceArray}
        =
        \begin{bNiceArray}{rrr}
            7/2 & 4 & 21/5
        \end{bNiceArray}
        \begin{bNiceArray}{r}
            2 \\
            3
        \end{bNiceArray}
        =
        43
    \]
    The sample covariance between $\textbf{b}^{\prime}\textbf{X}$ and $\textbf{c}^{\prime}\textbf{X}$
    \[
        \text{Sample covariance}
        =
        \text{Cov}(\textbf{c}^{\prime}\textbf{X}, \textbf{b}^{\prime}\textbf{X})
        =
        \textbf{c}^{\prime}\text{Cov}(\textbf{X}, \textbf{X})\textbf{b}
        =
        \textbf{c}^{\prime} V[\textbf{X}] \textbf{b}
        =
    \]
    \[
        =
        \textbf{c}^{\prime} \textbf{S}_{\textbf{X}} \textbf{b}
        =
        \begin{bNiceArray}{rrr}
            1 & 1 & 1
        \end{bNiceArray}
        \begin{bNiceArray}{rrr}
            13 & -5/2 & 3/2 \\
            -5/2 & 1 & -3/2 \\
            3/2 & -3/2 & 3
        \end{bNiceArray}
        \begin{bNiceArray}{r}
            1 \\
            2 \\
            -3
        \end{bNiceArray}
        =
    \]
    \[
        =
        \begin{bNiceArray}{rrr}
            12 & -3 & 3
        \end{bNiceArray}
        \begin{bNiceArray}{r}
            1 \\
            2 \\
            -3
        \end{bNiceArray}
        =
        12 - 6 - 9
        =
        -3
    \]
    Everything computed here in part (b) agrees with the corresponding values computed in part (a) using first principles.
\end{enumerate}