Given a data matrix $\textbf{X}$ and the resulting sample correlation matrix $\textbf{R}$,
consider the standardized observations $(x_{ik} - \bar{x}_{k})/\sqrt{s_{kk}}$, $k=1,2,\dots,p$,
$j=1,2,\dots,n$. Show that these standardized quantities have sample covariance
matrix $\textbf{R}$.
\newline
\par
Here are two solutions. One, using matrices and a second using the summations and algebra.
\newline
\underline{Solution 1:}
\[
    {[(x_{ik} - \bar{x}_{k})/\sqrt{s_{kk}}]}_{ik}
    =
    \left(\textbf{X} - \textbf{1}_{n}{\bar{\textbf{x}}}^{\prime}\right)\textbf{D}^{-1/2}
    =
    \textbf{X}_{\star}
\]
Use the formula for $\textbf{S}$ from (3-27),
\[
    \textbf{S}
    =
    \frac{1}{n-1}
    \textbf{X}_{\star}^{\prime}
    {\left(
        \textbf{I}
        -
        \frac{1}{n}
        \textbf{1}_{n}
        \textbf{1}_{n}^{\prime}
    \right)}
    \textbf{X}_{\star}
    =
\]
\[
    =
    \frac{1}{n-1}
    {\left(
        \left(\textbf{X} - \textbf{1}_{n}{\bar{\textbf{x}}}^{\prime}\right)\textbf{D}^{-1/2}
    \right)}^{\prime}
    {\left(
        \textbf{I}
        -
        \frac{1}{n}
        \textbf{1}_{n}
        \textbf{1}_{n}^{\prime}
    \right)}
    {\left(
        \left(\textbf{X} - \textbf{1}_{n}{\bar{\textbf{x}}}^{\prime}\right)\textbf{D}^{-1/2}
    \right)}
    =
\]
\[
    =
    \frac{1}{n-1}
    {\left(\textbf{D}^{-1/2}\right)}^{\prime}
    {\left(\textbf{X} - \textbf{1}_{n}{\bar{\textbf{x}}}^{\prime}\right)}^{\prime}
    {\left(
        \textbf{I}
        -
        \frac{1}{n}
        \textbf{1}_{n}
        \textbf{1}_{n}^{\prime}
    \right)}
    {\left(
        \left(\textbf{X} - \textbf{1}_{n}{\bar{\textbf{x}}}^{\prime}\right)\textbf{D}^{-1/2}
    \right)}
    =
\]
\[
    =
    \frac{1}{n-1}
    \textbf{D}^{-1/2}
    {\left(\textbf{X} - \textbf{1}_{n}{\bar{\textbf{x}}}^{\prime}\right)}^{\prime}
    {\left(
        \textbf{I}
        -
        \frac{1}{n}
        \textbf{1}_{n}
        \textbf{1}_{n}^{\prime}
    \right)}
    \left(\textbf{X} - \textbf{1}_{n}{\bar{\textbf{x}}}^{\prime}\right)\textbf{D}^{-1/2}
    =
\]
\[
    =
    \frac{1}{n-1}
    {\left(
        \textbf{D}^{-1/2}
        {\left(\textbf{X} - \textbf{1}_{n}{\bar{\textbf{x}}}^{\prime}\right)}^{\prime}
        \left(\textbf{X} - \textbf{1}_{n}{\bar{\textbf{x}}}^{\prime}\right)\textbf{D}^{-1/2}
        -
        \frac{1}{n}
        \textbf{D}^{-1/2}
        {\left(\textbf{X} - \textbf{1}_{n}{\bar{\textbf{x}}}^{\prime}\right)}^{\prime}
        \textbf{1}_{n}
        \textbf{1}_{n}^{\prime}
        \left(\textbf{X} - \textbf{1}_{n}{\bar{\textbf{x}}}^{\prime}\right)\textbf{D}^{-1/2}
    \right)}
    =
\]
\[
    =
    \frac{1}{n-1}
    {\left(
        \textbf{D}^{-1/2}
        ((n-1)\textbf{S})
        \textbf{D}^{-1/2}
        -
        \frac{1}{n}
        \textbf{D}^{-1/2}
        {\left(\textbf{X} - \textbf{1}_{n}{\bar{\textbf{x}}}^{\prime}\right)}^{\prime}
        \left(
            \textbf{1}_{n}
            \textbf{1}_{n}^{\prime}
            \textbf{X}
            - 
            \textbf{1}_{n}
            \textbf{1}_{n}^{\prime}
            \textbf{1}_{n}{\bar{\textbf{x}}}^{\prime}
        \right)
        \textbf{D}^{-1/2}
    \right)}
    =
\]
\[
    =
    \frac{1}{n-1}
    {\left(
        (n-1)
        \textbf{D}^{-1/2}
        \textbf{S}
        \textbf{D}^{-1/2}
        -
        \frac{1}{n}
        \textbf{D}^{-1/2}
        {\left(\textbf{X} - \textbf{1}_{n}{\bar{\textbf{x}}}^{\prime}\right)}^{\prime}
        \left(
            \textbf{1}_{n}
            \left(
                \textbf{1}_{n}^{\prime}
                \textbf{X}
            \right)
            - 
            \textbf{1}_{n}
            \left(
                \textbf{1}_{n}^{\prime}
                \textbf{1}_{n}
            \right)
            {\bar{\textbf{x}}}^{\prime}
        \right)
        \textbf{D}^{-1/2}
    \right)}
    =
\]
\[
    =
    \frac{1}{n-1}
    {\left(
        (n-1)
        \textbf{R}
        -
        \frac{1}{n}
        \textbf{D}^{-1/2}
        {\left(\textbf{X} - \textbf{1}_{n}{\bar{\textbf{x}}}^{\prime}\right)}^{\prime}
        \left(
            \textbf{1}_{n}
            \left(
                n
                {\bar{\textbf{x}}}^{\prime}
            \right)
            - 
            \textbf{1}_{n}
            \left(
                n
            \right)
            {\bar{\textbf{x}}}^{\prime}
        \right)
        \textbf{D}^{-1/2}
    \right)}
    =
\]
\[
    =
    \frac{1}{n-1}
    {\left(
        (n-1)
        \textbf{R}
        -
        \frac{1}{n}
        \textbf{D}^{-1/2}
        {\left(\textbf{X} - \textbf{1}_{n}{\bar{\textbf{x}}}^{\prime}\right)}^{\prime}
        \left(
            n
            \textbf{1}_{n}
            {\bar{\textbf{x}}}^{\prime}
            - 
            n
            \textbf{1}_{n}
            {\bar{\textbf{x}}}^{\prime}
        \right)
        \textbf{D}^{-1/2}
    \right)}
    =
\]
\[
    =
    \frac{1}{n-1}
    {\left(
        (n-1)
        \textbf{R}
        -
        \frac{1}{n}
        \textbf{D}^{-1/2}
        {\left(\textbf{X} - \textbf{1}_{n}{\bar{\textbf{x}}}^{\prime}\right)}^{\prime}
        0
        \textbf{D}^{-1/2}
    \right)}
    =
\]
\[
    =
    \frac{1}{n-1}
    {\left(
        (n-1)
        \textbf{R}
        -
        0
    \right)}
    =
\]
\[
    =
    \frac{n-1}{n-1}
    \textbf{R}
    =
\]
\[
    =
    \textbf{R}
\]
\underline{Solution 2:}
\newline
For an observation $j$ variable $k$, define the standardized values as
\[
    y_{jk} = \frac{x_{jk} - \bar{x}_{k}}{\sqrt{s_{kk}}}
\]
A mean value for variable $k$ from the $p$ by 1 mean vector would be
\[
    \bar{y}_{k}
    =
    \sum_{j=1}^{n}{\frac{y_{jk}}{n}}
    =
    \sum_{j=1}^{n}{\frac{(x_{jk} - \bar{x}_{k})}{n\sqrt{s_{kk}}}}
\]
An element $ik$ from the $p$ by $p$ covariance matrix would be
\[
    s_{ik}
    =
    \left(\frac{1}{n-1}\right)
    \sum_{j=1}^{n}\left(y_{ji} - \bar{y}_{i} \right)\left(y_{jk} - \bar{y}_{k} \right)
    =
\]
\[
    =
    \left(\frac{1}{n-1}\right)
    \sum_{j=1}^{n}\left(\left(\frac{x_{ji} - \bar{x}_{i}}{\sqrt{s_{ii}}}\right) - \left(\sum_{\ell=1}^{n}{\frac{(x_{\ell i} - \bar{x}_{i})}{n\sqrt{s_{ii}}}}\right) \right)\left(\left(\frac{x_{jk} - \bar{x}_{k}}{\sqrt{s_{kk}}}\right) - \left(\sum_{\ell=1}^{n}{\frac{(x_{\ell k} - \bar{x}_{k})}{n\sqrt{s_{kk}}}}\right) \right)
    =
\]
\[
    =
    \left(\frac{1}{n-1}\right)
    \left(\frac{1}{\sqrt{s_{ii}}\sqrt{s_{kk}}}\right)
    \sum_{j=1}^{n}
    \left(x_{ji} - \bar{x}_{i} - \left(\sum_{\ell=1}^{n}{\frac{x_{\ell i} - \bar{x}_{i}}{n}}\right) \right)
    \left(x_{jk} - \bar{x}_{k} - \left(\sum_{\ell=1}^{n}{\frac{x_{\ell k} - \bar{x}_{k}}{n}}\right) \right)
    =
\]
\[
    =
    \left(\frac{1}{n-1}\right)
    \left(\frac{1}{\sqrt{s_{ii}}\sqrt{s_{kk}}}\right)
    \sum_{j=1}^{n}
    \left(x_{ji} - \bar{x}_{i} - \left(\sum_{\ell=1}^{n}{\frac{x_{\ell i}}{n}}\right) + n\frac{\bar{x}_{i}}{n} \right)
    \left(x_{jk} - \bar{x}_{k} - \left(\sum_{\ell=1}^{n}{\frac{x_{\ell k}}{n}}\right) - n\frac{\bar{x}_{k}}{n} \right)
    =
\]
\[
    =
    \left(\frac{1}{n-1}\right)
    \left(\frac{1}{\sqrt{s_{ii}}\sqrt{s_{kk}}}\right)
    \sum_{j=1}^{n}
    \left(x_{ji} - \bar{x}_{i} - \bar{x}_{i} + \bar{x}_{i} \right)
    \left(x_{jk} - \bar{x}_{k} - \bar{x}_{k} + \bar{x}_{k} \right)
    =
\]
\[
    =
    \left(\frac{1}{n-1}\right)
    \left(\frac{1}{\sqrt{s_{ii}}\sqrt{s_{kk}}}\right)
    \sum_{j=1}^{n}
    \left(x_{ji} - \bar{x}_{i} \right)
    \left(x_{jk} - \bar{x}_{k} \right)
    =
\]
\[
    =
    \left(\frac{1}{n-1}\right)
    \left(\frac{1}{\sqrt{s_{ii}}\sqrt{s_{kk}}}\right)
    (n-1)s_{ik}
    =
\]
\[
    =
    \frac{s_{ik}}{\sqrt{s_{ii}}\sqrt{s_{kk}}}
    =
    r_{ik}
\]
This is element $ik$ from the $p$ by $p$ sample correlation matrix.
