Consider the data matrix $\textbf{X}$ in Exercise 3.1. 
We have $n = 3$ observations on $p = 2$ variables $X_1$ and $X_2$. 
Form the linear combinations
\[
    \textbf{c}^{\prime}\textbf{X}
    =
    \begin{bNiceArray}{cc}
        -1 & 2
    \end{bNiceArray}
    \begin{bNiceArray}{c}
        X_1 \\
        X_2
    \end{bNiceArray}
    =
    - X_1 + 2X_2
\]
\[
    \textbf{b}^{\prime}\textbf{X}
    =
    \begin{bNiceArray}{cc}
        2 & 3
    \end{bNiceArray}
    \begin{bNiceArray}{c}
        X_1 \\
        X_2
    \end{bNiceArray}
    =
    2X_1 + 3X_2
\]
\begin{enumerate}[label=(\alph*)]
    \item Evaluate the sample means, variances, and covariance of $\textbf{b}^{\prime}\textbf{X}$ and $\textbf{c}^{\prime}\textbf{X}$ from first principles. That is, calculate the observed values of $\textbf{b}^{\prime}\textbf{X}$ and $\textbf{c}^{\prime}\textbf{X}$ and then use the sample mean, variance, and covariance formulas.
    \[
        \textbf{X}
        =
        \begin{bNiceArray}{cc}
            9 & 1 \\
            5 & 3 \\
            1 & 2
        \end{bNiceArray}
    \]
    \[
        \begin{NiceArray}{l}
            \textbf{c}^{\prime}\textbf{x}_1 = -1x_{11} + 2x_{12} = -1(9) + 2(1) = -7 \\
            \textbf{c}^{\prime}\textbf{x}_2 = -1x_{21} + 2x_{22} = -1(5) + 2(3) = 1 \\
            \textbf{c}^{\prime}\textbf{x}_3 = -1x_{31} + 2x_{32} = -1(1) + 2(2) = 3 \\
        \end{NiceArray}
    \]
    \[
        \text{Sample mean}
        =
        \frac{(-7 + 1 + 3)}{3}
        =
        -1
    \]
    \[
        \text{Sample variance}
        =
        \frac{{(-7 + 1)}^2
        +
        {(1 + 1)}^2
        +
        {(3 + 1)}^2
        }{3 - 1}
        =
        28
    \]
    \[
        \begin{NiceArray}{l}
            \textbf{b}^{\prime}\textbf{x}_1 = 2x_{11} + 3x_{12} = 2(9) + 3(1) = 21 \\
            \textbf{b}^{\prime}\textbf{x}_2 = 2x_{21} + 3x_{22} = 2(5) + 3(3) = 19 \\
            \textbf{b}^{\prime}\textbf{x}_3 = 2x_{31} + 3x_{32} = 2(1) + 3(2) = 8 \\
        \end{NiceArray}
    \]
    \[
        \text{Sample mean}
        =
        \frac{(21 + 19 + 8)}{3}
        =
        16
    \]
    \[
        \text{Sample variance}
        =
        \frac{{(21 - 16)}^2
        +
        {(19 - 16)}^2
        +
        {(8 - 16)}^2
        }{3 - 1}
        =
        49
    \]
    The covariance between $\textbf{b}^{\prime}\textbf{X}$ and $\textbf{c}^{\prime}\textbf{X}$
    \[
        \text{Sample covariance}
        =
    \]
    \[
        =
        \frac{(-7 + 1)(21 - 16)
        +
        (1 + 1)(19 - 16)
        +
        (3 + 1)(8 - 16)
        }{3 - 1}
        =
    \]
    \[
        =
        -28
    \]
    \item Calculate the sample means, variances, covariance of $\textbf{B}^{\prime}\textbf{X}$ and $\textbf{c}^{\prime}\textbf{X}$ using (3-36). Compare the results in (a) and (b).
    \newline
    \par
    First, compute $\bar{\textbf{x}}$ and $\textbf{S}_{\textbf{X}}$
    \[
        \bar{\textbf{x}}
        =
        \frac{1}{n} \textbf{X}^{\prime} \textbf{1}_n
        =
        \frac{1}{3} \textbf{X}^{\prime} \textbf{1}_3
        =
        \frac{1}{3}
        \begin{bNiceArray}{ccc}
            9 & 5 & 1 \\
            1 & 3 & 2
        \end{bNiceArray}
        \begin{bNiceArray}{c}
            1 \\
            1 \\
            1
        \end{bNiceArray}
        =
        \frac{1}{3}
        \begin{bNiceArray}{c}
            15 \\
            6
        \end{bNiceArray}
        =
        \begin{bNiceArray}{c}
            5 \\
            2
        \end{bNiceArray}
    \]
    The deviance is
    \[
        \textbf{X} - \textbf{1}_n \bar{\textbf{x}}^{\prime}
        =
        \textbf{X} - \textbf{1}_3 \bar{\textbf{x}}^{\prime}
        =
        \begin{bNiceArray}{cc}
            9 & 1 \\
            5 & 3 \\
            1 & 2
        \end{bNiceArray}
        -
        \begin{bNiceArray}{cc}
            1 \\
            1 \\
            1
        \end{bNiceArray}
        \begin{bNiceArray}{cc}
            5 & 2 \\
        \end{bNiceArray}
        =
    \]
    \[
        =
        \begin{bNiceArray}{cc}
            9 & 1 \\
            5 & 3 \\
            1 & 2
        \end{bNiceArray}
        -
        \begin{bNiceArray}{cc}
            5 & 2 \\
            5 & 2 \\
            5 & 2
        \end{bNiceArray}
        =
        \begin{bNiceArray}{rr}
            4 & -1 \\
            0 & 1 \\
            -4 & 0
        \end{bNiceArray}
    \]
    Using the deviance to get $\textbf{S}_{\textbf{X}}$
    \[
        \textbf{S}_{\textbf{X}}
        =
        \left(\frac{1}{n - 1}\right)
        {\left(\textbf{X} - \textbf{1}_n \bar{\textbf{x}}^{\prime}\right)}^{\prime}
        \left(\textbf{X} - \textbf{1}_n \bar{\textbf{x}}^{\prime}\right)
        =
    \]
    \[
        =
        \left(\frac{1}{3 - 1}\right)
        \begin{bNiceArray}{rrr}
            4 & 0 & -4 \\
            -1 & 1 & 0
        \end{bNiceArray}
        \begin{bNiceArray}{rr}
            4 & -1 \\
            0 & 1 \\
            -4 & 0
        \end{bNiceArray}
        =
    \]
    \[
        =
        \left(\frac{1}{3 - 1}\right)
        \begin{bNiceArray}{rr}
            32 & -4 \\
            -4 & 2
        \end{bNiceArray}
        =
        \begin{bNiceArray}{rr}
            16 & -2 \\
            -2 & 1
        \end{bNiceArray}
    \]
    \[
        \text{sample mean}
        =
        E[\textbf{c}^{\prime}\textbf{X}]
        =
        \textbf{c}^{\prime} E[\textbf{X}]
        =
        \textbf{c}^{\prime} \bar{\textbf{x}}
        =
        \begin{bNiceArray}{rr}
            -1 & 2
        \end{bNiceArray}
        \begin{bNiceArray}{c}
            5 \\
            2
        \end{bNiceArray}
        =
        -5+4
        =
        -1
    \]
    \[
        \text{sample variance}
        =
        V[\textbf{c}^{\prime}\textbf{X}]
        =
        \textbf{c}^{\prime} V[\textbf{X}]\textbf{c}
        =
        \textbf{c}^{\prime} \textbf{S}_{\textbf{X}} \textbf{c}
        =
    \]
    \[
        =
        \begin{bNiceArray}{rr}
            -1 & 2
        \end{bNiceArray}
        \begin{bNiceArray}{rr}
            16 & -2 \\
            -2 & 1
        \end{bNiceArray}
        \begin{bNiceArray}{r}
            -1 \\
            2
        \end{bNiceArray}
        =
        \begin{bNiceArray}{rr}
            -20 & 4
        \end{bNiceArray}
        \begin{bNiceArray}{r}
            -1 \\
            2
        \end{bNiceArray}
        =
        28
    \]
    \[
        \text{sample mean}
        E[\textbf{b}^{\prime}\textbf{X}]
        =
        \textbf{b}^{\prime} E[\textbf{X}]
        =
        \textbf{b}^{\prime} \bar{\textbf{x}}
        =
        \begin{bNiceArray}{rr}
            2 & 3
        \end{bNiceArray}
        \begin{bNiceArray}{c}
            5 \\
            2
        \end{bNiceArray}
        =
        10+6
        =
        16
    \]
    \[
        \text{sample variance}
        =
        V[\textbf{b}^{\prime}\textbf{X}]
        =
        \textbf{b}^{\prime} V[\textbf{X}] \textbf{c}
        =
        \textbf{b}^{\prime} \textbf{S}_{\textbf{X}} \textbf{c}
        =
    \]
    \[
        =
        \begin{bNiceArray}{rr}
            2 & 3
        \end{bNiceArray}
        \begin{bNiceArray}{rr}
            16 & -2 \\
            -2 & 1
        \end{bNiceArray}
        \begin{bNiceArray}{r}
            2 \\
            3
        \end{bNiceArray}
        =
        \begin{bNiceArray}{rr}
            26 & -1
        \end{bNiceArray}
        \begin{bNiceArray}{r}
            2 \\
            3
        \end{bNiceArray}
        =
        49
    \]
    The sample covariance between $\textbf{b}^{\prime}\textbf{X}$ and $\textbf{c}^{\prime}\textbf{X}$
    \[
        \text{Sample covariance}
        =
        \text{Cov}(\textbf{c}^{\prime}\textbf{X}, \textbf{b}^{\prime}\textbf{X})
        =
        \textbf{c}^{\prime}\text{Cov}(\textbf{X}, \textbf{X})\textbf{b}
        =
        \textbf{c}^{\prime} V[\textbf{X}] \textbf{b}
        =
        \textbf{c}^{\prime} \textbf{S}_{\textbf{X}} \textbf{b}
        =
    \]
    \[
        =
        \begin{bNiceArray}{rr}
            -1 & 2
        \end{bNiceArray}
        \begin{bNiceArray}{rr}
            16 & -2 \\
            -2 & 1
        \end{bNiceArray}
        \begin{bNiceArray}{r}
            2 \\
            3
        \end{bNiceArray}
        =
        \begin{bNiceArray}{rr}
            -20 & 4
        \end{bNiceArray}
        \begin{bNiceArray}{r}
            2 \\
            3
        \end{bNiceArray}
        =
        -40 + 12
        =
        -28
    \]
    Everything computed here in part (b) agrees with the corresponding values computed in part (a) using first principles.
\end{enumerate}