Let $\textbf{V}$ be a vector random variable with mean vector $E(\textbf{V}) = \bm{\mu}_{\textbf{V}}$ and covariance matrix $E(\textbf{V}-\bm{\mu}_{\textbf{V}}){(\textbf{V}-\bm{\mu}_{\textbf{V}})}^{\prime} = \bm{\Sigma}_{\textbf{V}}$. Show that $E(\textbf{V}{\textbf{V}}^{\prime}) = \bm{\Sigma}_{\textbf{V}} + \bm{\mu}_{\textbf{V}}{\bm{\mu}_{\textbf{V}}}^{\prime}$.
\[
    \bm{\Sigma}_{\textbf{V}}
    =
    E(\textbf{V}-\bm{\mu}_{\textbf{V}}){(\textbf{V}-\bm{\mu}_{\textbf{V}})}^{\prime}
    =
    E(\textbf{V}-\bm{\mu}_{\textbf{V}})(\textbf{V}^{\prime}-\bm{\mu}_{\textbf{V}}^{\prime})
    =
\]
\[
    =
    E
    \left[
        \textbf{V}
        \textbf{V}^{\prime}
        -
        \textbf{V}
        \bm{\mu}_{\textbf{V}}^{\prime}
        -
        \bm{\mu}_{\textbf{V}}
        \textbf{V}^{\prime}
        +
        \bm{\mu}_{\textbf{V}}
        \bm{\mu}_{\textbf{V}}^{\prime}
    \right]
    =
\]
\[
    =
    E \left[
        \textbf{V}
        \textbf{V}^{\prime}
    \right]
    -
    E \left[
        \textbf{V}
        \bm{\mu}_{\textbf{V}}^{\prime}
    \right]
    -
    E \left[
        \bm{\mu}_{\textbf{V}}
        \textbf{V}^{\prime}
    \right]
    +
    E \left[
        \bm{\mu}_{\textbf{V}}
        \bm{\mu}_{\textbf{V}}^{\prime}
    \right]
    =
\]
\[
    =
    E \left[
        \textbf{V}
        \textbf{V}^{\prime}
    \right]
    -
    E \left[
        \textbf{V}
    \right]
    \bm{\mu}_{\textbf{V}}^{\prime}
    -
    \bm{\mu}_{\textbf{V}}
    E \left[
        \textbf{V}^{\prime}
    \right]
    +
    \bm{\mu}_{\textbf{V}}
    \bm{\mu}_{\textbf{V}}^{\prime}
    =
\]
\[
    =
    E \left[
        \textbf{V}
        \textbf{V}^{\prime}
    \right]
    -
    \bm{\mu}_{\textbf{V}}
    \bm{\mu}_{\textbf{V}}^{\prime}
    -
    \bm{\mu}_{\textbf{V}}
    \bm{\mu}_{\textbf{V}}^{\prime}
    +
    \bm{\mu}_{\textbf{V}}
    \bm{\mu}_{\textbf{V}}^{\prime}
    =
\]
\[
    =
    E \left[
        \textbf{V}
        \textbf{V}^{\prime}
    \right]
    -
    \bm{\mu}_{\textbf{V}}
    \bm{\mu}_{\textbf{V}}^{\prime}
    =
    \bm{\Sigma}_{\textbf{V}}
\]
\[
    \Rightarrow
    E \left[
        \textbf{V}
        \textbf{V}^{\prime}
    \right]
    =
    \bm{\Sigma}_{\textbf{V}}
    +
    \bm{\mu}_{\textbf{V}}
    \bm{\mu}_{\textbf{V}}^{\prime}
\]