Consider the univariate one-way decomposition of the observation $x_{\ell j}$ given by (6--34).
Show that the mean vector $\bar{x}\textbf{1}$ is always perpendicular to the treatment effect vector
$(\bar{x}_{1} - \bar{x})\textbf{u}_{1} + (\bar{x}_{2} - \bar{x})\textbf{u}_{2} + \cdots + (\bar{x}_{g} - \bar{x})\textbf{u}_{\text{g}}$ where 

\[
    \begin{NiceMatrix}
        \Block{9-1}{\textbf{u}_{1} = }
        & 1
        & \Block{3-1}{\quad n_{1}}
        & \Block{9-1}{,}
        & \Block{9-1}{\textbf{u}_{2} = }
        & 0
        & \Block{9-1}{\quad n_{2}}
        & \Block{9-1}{, \dots,}
        & \Block{9-1}{\textbf{u}_{\text{g}} = }
        & 0
        & \Block{9-1}{
            \quad \phantom{0} \\
            \quad \phantom{\vdots} \\
            \quad \phantom{0} \\
            \quad \phantom{0} \\
            \quad \phantom{\vdots} \\
            \quad \phantom{0} \\
            \quad \phantom{1} \\
            \quad n_{\text{g}} \phantom{\vdots}\\
            \quad \phantom{0}
            } \\
        & \vdots &  &  &  & \vdots &  &  &  & \vdots \\
        & 1      &  &  &  & 0      &  &  &  & 0      \\
        & 0      &  &  &  & 1      &  &  &  & 0      \\
        & \vdots &  &  &  & \vdots &  &  &  & \vdots \\
        & 0      &  &  &  & 1      &  &  &  & 0      \\
        & 0      &  &  &  & 0      &  &  &  & 1      \\
        & \vdots &  &  &  & \vdots &  &  &  & \vdots \\
        & 0      &  &  &  & 0      &  &  &  & 1 
        \CodeAfter
        % Draw square brackets around the array.
        \SubMatrix[{1-2}{9-2}]
        \SubMatrix[{1-6}{9-6}]
        \SubMatrix[{1-10}{9-10}]
        % Draw the right brace for the first three rows.
        \SubMatrix{.}{1-2}{3-2}{\}}[xshift=2mm]
        \SubMatrix{.}{4-6}{6-6}{\}}[xshift=2mm]
        \SubMatrix{.}{7-10}{9-10}{\}}[xshift=2mm]
    \end{NiceMatrix}
\]

An $r \times c$ matrix of 1s is denoted $\textbf{1}_{r}^{c}$.

Also, $n = \sum_{\ell=1}^{\text{g}}{n_{\ell}}$ and $\sum_{\ell=1}^{\text{g}}
\sum_{j=1}^{n_{\ell}}
{x_{\ell j}}/n = \bar{x}$.
The dot product between the vectors of interest is

\[
    \bar{x} \textbf{1}_{n}
    \cdot
    [
        (\bar{x}_{1} - \bar{x}) \textbf{u}_{1}
        +
        (\bar{x}_{2} - \bar{x}) \textbf{u}_{2}
        + \cdots +
        (\bar{x}_{g} - \bar{x}) \textbf{u}_{\text{g}}
    ]
    =
\]
\[
    =
    n_{1} \bar{x} (\bar{x}_{1} - \bar{x})
    +
    n_{2} \bar{x} (\bar{x}_{2} - \bar{x})
    + \cdots +
    n_{\text{g}} \bar{x} (\bar{x}_{g} - \bar{x})
=
\]
\[
    =
    \sum_{\ell=1}^{\text{g}}
    {
        n_{\ell} \bar{x} (\bar{x}_{\ell} - \bar{x})
    }
    =
    \sum_{\ell=1}^{\text{g}}
    {
        \left(
            n_{\ell} \bar{x} \bar{x}_{\ell}
            -
            n_{\ell} \bar{x}^{2}
        \right)
    }
    =
    \bar{x}
    \sum_{\ell=1}^{\text{g}}
    {n_{\ell} \bar{x}_{\ell}}
        -
    \bar{x}^{2}
    \sum_{\ell=1}^{\text{g}}
    {n_{\ell}}
    =
\]
\[
    =
    \bar{x}
    \sum_{\ell=1}^{\text{g}}
    \sum_{j=1}^{n_{\ell}}
    {x_{\ell j}}
    -
    n\bar{x}^{2}
    =
    n\bar{x}^{2}
    -
    n\bar{x}^{2}
    =
    0
\]
