Let $\textbf{X}_{1},\textbf{X}_{2},\dots,\textbf{X}_{20}$ be a random sample of size $n = 20$ from a $N_{6}(\bm{\mu},\bm{\Sigma})$ population. Specify each of the following completely.
\begin{enumerate}[label= (\alph*)]
    \item The distribution of ${(\textbf{X}_1 - \bm{\mu})}^{\prime}\bm{\Sigma}^{-1}(\textbf{X}_1 - \bm{\mu})$
    \newline
    Can use Result 4.7 (a) on page 163 for this
    \[
        {(\textbf{X}_1 - \bm{\mu})}^{\prime}\bm{\Sigma}^{-1}(\textbf{X}_1 - \bm{\mu})
        \sim
        \mathlarger{\chi_{6}^{2}}
    \]
    \item The distribution of $\bar{\textbf{X}}$ and $\sqrt{n}(\bar{\textbf{X}} - \bm{\mu})$
    \[
        \textbf{Y}_{1}
        =
        \bar{\textbf{X}}
        =
        \begin{bNiceArray}{c}
            \bar{\textbf{x}}_{1} \\
            \vdots \\
            \bar{\textbf{x}}_{6}
        \end{bNiceArray}
        =
        \left(
            \textbf{X}_{1} +
            \cdots +
            \textbf{X}_{20}
        \right) / 20
        =
        \frac{\sum_{j=1}^{20}\textbf{X}_{j}}{20}
    \]
    \[
        \text{E}
        \left[
            \textbf{Y}_{1}
        \right]
        =
        \text{E}
        \left[
            \frac{\sum_{j=1}^{20}\textbf{X}_{j}}{20}
        \right]
        =
        \frac{\sum_{j=1}^{20}\text{E}\left[\textbf{X}_{j}\right]}{20}
        =
        \frac{\sum_{j=1}^{20}\bm{\mu}}{20}
        =
        \frac{20\bm{\mu}}{20}
        =
        \bm{\mu}
    \]
    \[
        \text{Covar}
        \left[
            \textbf{Y}_{1}
        \right]
        =
        \text{Covar}
        \left[
            \frac{\sum_{j=1}^{20}\textbf{X}_{j}}{20}
        \right]
        =
        {\left(\frac{1}{{20}}\right)}^{2}\sum_{j=1}^{20}{\text{Covar}\left[\textbf{X}_{j}\right]}
        =
    \]
    \[
        {\left(\frac{1}{{20}}\right)}^{2}\left(\sum_{j=1}^{20}{\bm{\Sigma}}\right)
        =
        {\left(\frac{1}{{20}}\right)}^{2}\left(20\bm{\Sigma}\right)
        =
        \frac{1}{20}\bm{\Sigma}
    \]
    \[
        \textbf{Y}_{1}
        =
        \bar{\textbf{X}}
        \sim
        N_{6}\left(\bm{\mu}, \frac{1}{20}\bm{\Sigma}\right)
    \]
    This is the same as (4--23) in section 4.4 on page 174.
    \newline
    If $\textbf{Y}_{2} = \sqrt{n}(\bar{\textbf{X}} - \bm{\mu})$, then
    \[
        \text{E}
        \left[
            \textbf{Y}
        \right]
        =
        \text{E}
        \left[
            \sqrt{n}(\bar{\textbf{X}} - \bm{\mu})
        \right]
        =
        \text{E}\left[\sqrt{n}\bar{\textbf{X}}\right]
        -
        \text{E}\left[\sqrt{n}\bm{\mu}\right]
        =
        \text{E}\left[\sqrt{n}\bar{\textbf{X}}\right]
        -
        \text{E}\left[\sqrt{n}\bm{\mu}\right]
        =
    \]
    \[
        =
        \sqrt{n}\text{E}\left[\bar{\textbf{X}}\right]
        -
        \sqrt{n}\bm{\mu}
        =
        \sqrt{n}\bm{\mu}
        -
        \sqrt{n}\bm{\mu}
        =
        \textbf{0}
    \]
    \[
        \text{Covar}
        \left[
            \textbf{Y}_{2}
        \right]
        =
        \text{Covar}
        \left[
            \sqrt{n}(\bar{\textbf{X}} - \bm{\mu})
        \right]
        =
        \text{Covar}\left[\sqrt{n}\bar{\textbf{X}}\right] - \text{Covar}\left[\sqrt{n}\bm{\mu}\right]
        =
    \]
    \[
        =
        {\left(\sqrt{n}\right)}^{2}\text{Covar}\left[\bar{\textbf{X}}\right] - \textbf{0}
        =
        n\left(\frac{1}{n}\bm{\Sigma}\right)
        =
        \bm{\Sigma}
    \]
    \[
        \textbf{Y}_{2}
        =
        \sqrt{n}(\bar{\textbf{X}} - \bm{\mu})
        \sim
        N_{6}\left(\textbf{0},\bm{\Sigma}\right)
    \]
    This is the same as the approximation in (4--28) in section 4.5 on page 176.
    \item The distribution of (n-1)\textbf{S}
    \[
        (n-1)\textbf{S}
        =
        \frac{n-1}{n -1}
        \sum_{j=1}^{n}{
            \left(\textbf{X}_{j} - \bar{\textbf{X}}\right)
            {\left(\textbf{X}_{j} - \bar{\textbf{X}}\right)}^{\prime}
        }
        =
    \]
    \[
        =
        \sum_{j=1}^{n}{
            \left(\textbf{X}_{j} + \bm{\mu} - \bm{\mu} - \bar{\textbf{X}}\right)
            {\left(\textbf{X}_{j} + \bm{\mu} - \bm{\mu} - \bar{\textbf{X}}\right)}^{\prime}
        }
        =
    \]
    \[
        =
        \sum_{j=1}^{n}{
            \left((\textbf{X}_{j} - \bm{\mu}) - (\bar{\textbf{X}} - \bm{\mu})\right)
            {\left((\textbf{X}_{j} - \bm{\mu}) - (\bar{\textbf{X}} - \bm{\mu})\right)}^{\prime}
        }
        =
    \]
    \[
        =
        \scriptstyle{
        \sum_{j=1}^{n}{
            (\textbf{X}_{j} - \bm{\mu}){(\textbf{X}_{j} - \bm{\mu})}^{\prime}
            -
            (\bar{\textbf{X}} - \bm{\mu}){(\textbf{X}_{j} - \bm{\mu})}^{\prime}
            -
            (\textbf{X}_{j} - \bm{\mu}){(\bar{\textbf{X}} - \bm{\mu})}^{\prime}
            +
            (\bar{\textbf{X}} - \bm{\mu}){(\bar{\textbf{X}} - \bm{\mu})}^{\prime}
        }
        }
        =
    \]
    \[
        =
        \scriptstyle{
        \sum_{j=1}^{n}{
            (\textbf{X}_{j} - \bm{\mu}){(\textbf{X}_{j} - \bm{\mu})}^{\prime}
        }
        -
        2
        \sum_{j=1}^{n}{
            (\textbf{X}_{j} - \bm{\mu}){(\bar{\textbf{X}} - \bm{\mu})}^{\prime}
        }
        +
        \sum_{j=1}^{n}{
            (\bar{\textbf{X}} - \bm{\mu}){(\bar{\textbf{X}} - \bm{\mu})}^{\prime}
        }
        }
        =
    \]
    \[
        =
        \scriptstyle{
        \sum_{j=1}^{n}{
            (\textbf{X}_{j} - \bm{\mu}){(\textbf{X}_{j} - \bm{\mu})}^{\prime}
        }
        -
        2
        (\bar{\textbf{X}} - \bm{\mu})
        \sum_{j=1}^{n}{
            {(\textbf{X}_{j} - \bm{\mu})}^{\prime}
        }
        +
        n
        (\bar{\textbf{X}} - \bm{\mu}){(\bar{\textbf{X}} - \bm{\mu})}^{\prime}
        }
        =
    \]
    \[
        =
        \scriptstyle{
        \sum_{j=1}^{n}{
            (\textbf{X}_{j} - \bm{\mu}){(\textbf{X}_{j} - \bm{\mu})}^{\prime}
        }
        -
        2
        (\bar{\textbf{X}} - \bm{\mu})
        {((\sum_{j=1}^{n}{\textbf{X}_{j}}) - n\bm{\mu})}^{\prime}
        +
        n
        (\bar{\textbf{X}} - \bm{\mu}){(\bar{\textbf{X}} - \bm{\mu})}^{\prime}
        }
        =
    \]
    \[
        =
        \scriptstyle{
        \sum_{j=1}^{n}{
            (\textbf{X}_{j} - \bm{\mu}){(\textbf{X}_{j} - \bm{\mu})}^{\prime}
        }
        -
        2
        (\bar{\textbf{X}} - \bm{\mu})
        {(n\bar{\textbf{X}} - n\bm{\mu})}^{\prime}
        +
        n
        (\bar{\textbf{X}} - \bm{\mu}){(\bar{\textbf{X}} - \bm{\mu})}^{\prime}
        }
        =
    \]
    \[
        =
        \scriptstyle{
        \sum_{j=1}^{n}{
            (\textbf{X}_{j} - \bm{\mu}){(\textbf{X}_{j} - \bm{\mu})}^{\prime}
        }
        -
        2n
        (\bar{\textbf{X}} - \bm{\mu})
        {(\bar{\textbf{X}} - \bm{\mu})}^{\prime}
        +
        n
        (\bar{\textbf{X}} - \bm{\mu}){(\bar{\textbf{X}} - \bm{\mu})}^{\prime}
        }
        =
    \]
    \[
        =
        \sum_{j=1}^{n}{
            (\textbf{X}_{j} - \bm{\mu}){(\textbf{X}_{j} - \bm{\mu})}^{\prime}
        }
        -
        n
        (\bar{\textbf{X}} - \bm{\mu})
        {(\bar{\textbf{X}} - \bm{\mu})}^{\prime}
        =
    \]
    \[
        =
        \sum_{j=1}^{n}{
            (\textbf{X}_{j} - \bm{\mu}){(\textbf{X}_{j} - \bm{\mu})}^{\prime}
        }
        -
        \left[
            \sqrt{n}
            (\bar{\textbf{X}} - \bm{\mu})
        \right]
        \left[
            \sqrt{n}
            {(\bar{\textbf{X}} - \bm{\mu})}^{\prime}
        \right]
        =
    \]
    so looking at the first and second part of this equation
    \[
        \textbf{X}_{j}
        \sim
        N(\underset{(p \times 1)}{\bm{\mu}}, \underset{(p \times p)}{\bm{\Sigma}})
        \hspace{0.2cm}
        \Rightarrow
        \hspace{0.2cm}
        (\textbf{X}_{j} - \bm{\mu})
        \sim
        N(\textbf{0}, \Sigma)
        \Rightarrow
    \]
    \[
        \Rightarrow
        (\textbf{X}_{j} - \bm{\mu}){(\textbf{X}_{j} - \bm{\mu})}^{\prime}
        \sim
        \chi_{1}^{2}
        \Rightarrow
    \]
    \[
        \Rightarrow
        \sum_{j=1}^{n}{
            (\textbf{X}_{j} - \bm{\mu}){(\textbf{X}_{j} - \bm{\mu})}^{\prime}
        }
        \sim
        W_{n}(\Sigma)
    \]
    That is, the first term in the sum is distributed as a Wishart distribution with $n$ degrees of freedom. For the second term,
    \[
        \bar{\textbf{X}}
        \sim
        N(\bm{\mu}, \bm{\Sigma}/n)
        \Rightarrow
        (\bar{\textbf{X}} - \bm{\mu})
        \sim
        N(\textbf{0}, \bm{\Sigma}/n)
        \Rightarrow
    \]
    \[
        \Rightarrow
        \sqrt{n}
        (\bar{\textbf{X}} - \bm{\mu})
        \sim
        N(\textbf{0}, \bm{\Sigma})
        \Rightarrow
    \]
    \[
        \left[
            \sqrt{n}
            (\bar{\textbf{X}} - \bm{\mu})
        \right]
        \left[
            \sqrt{n}
            {(\bar{\textbf{X}} - \bm{\mu})}^{\prime}
        \right]
        \sim
        W_{1}(\bm{\Sigma})
    \]
    That is, the second term in the sum is distributed as a Wishart distribution with 1 degree of freedom.

    Combining the two, we now has a Wishart distribution with $n$ degrees of freedom minus another Wishart distribution with 1 degree of freedom to create a Wishart distribution with $n - 1$ distribution, so we finally have
    \[
        (n-1)\textbf{S}
        \sim
        W_{n-1}\left(\underset{(p \times p)}{\bm{\Sigma}}\right)
    \]
    This is the answers found in (4--23) on page 174. For this data we have
    \[
        (n-1)\textbf{S}
        \sim
        W_{20-1}\left(\underset{(6 \times 6)}{\bm{\Sigma}}\right)
    \]
    A Wishart distribution with 19 degrees of freedom.
    
\end{enumerate}