Show that $\sum_{j=1}^{n}{(\textbf{x}_{j} - \bar{\textbf{x}}){(\bar{\textbf{x}} - \bm{\mu})}^{\prime}}$ and $\sum_{j=1}^{n}{(\bar{\textbf{x}} - \bm{\mu}){(\textbf{x}_{j} - \bar{\textbf{x}})}^{\prime}}$ are both $p \times p$ matrices of zeros. Here $\textbf{x}_{j}^{\prime} = [x_{j1}, x_{j2}, \dots, x_{jp}]$, $j=1,2,\dots,n$ and
\[
    \bar{\textbf{x}}
    =
    \frac{1}{n}
    \sum_{j=1}^{n}{\textbf{x}_{j}}
\]
Here are both a short answer (using distribution and vector-vector multiplication) and long ugly answer (multiply matrix out).
\newline
\underline{Short answer:}
\[
    \sum_{j=1}^{n}{
        (\textbf{x}_{j} - \bar{\textbf{x}})
        {(\bar{\textbf{x}} - \bm{\mu})}^{\prime}
    }
    =
\]
\[
    =
    \sum_{j=1}^{n}{
        (\textbf{x}_{j} - \bar{\textbf{x}})
        {(\bar{\textbf{x}}^{\prime} - \bm{\mu}^{\prime})}
    }
    =
\]
\[
    =
    \sum_{j=1}^{n}{
        \left(
            \underset{(p \times 1)}{\textbf{x}_{j}}
            \underset{(1 \times p)}{\bar{\textbf{x}}^{\prime}}
            -
            \underset{(p \times 1)}{\bar{\textbf{x}}}
            \underset{(1 \times p)}{\bar{\textbf{x}}^{\prime}}
            -
            \underset{(p \times 1)}{\textbf{x}_{j}}
            \underset{(1 \times p)}{\bm{\mu}^{\prime}}
            +
            \underset{(p \times 1)}{\bar{\textbf{x}}}
            \underset{(1 \times p)}{\bm{\mu}^{\prime}}
        \right)
    }
    =
\]
\[
    =
    \sum_{j=1}^{n}{
        \left(
            \underset{(p \times 1)}{\textbf{x}_{j}}
            \underset{(1 \times p)}{\bar{\textbf{x}}^{\prime}}
        \right)
    }
    -
    n
    \underset{(p \times 1)}{\bar{\textbf{x}}}
    \underset{(1 \times p)}{\bar{\textbf{x}}^{\prime}}
    -
    \sum_{j=1}^{n}{
        \left(
            \underset{(p \times 1)}{\textbf{x}_{j}}
            \underset{(1 \times p)}{\bm{\mu}^{\prime}}
        \right)
    }
    +
    n
    \underset{(p \times 1)}{\bar{\textbf{x}}}
    \underset{(1 \times p)}{\bm{\mu}^{\prime}}
    =
\]
\[
    =
    n
    \underset{(p \times 1)}{\bar{\textbf{x}}}
    \underset{(1 \times p)}{\bar{\textbf{x}}^{\prime}}
    -
    n
    \underset{(p \times 1)}{\bar{\textbf{x}}}
    \underset{(1 \times p)}{\bar{\textbf{x}}^{\prime}}
    -
    n
    \underset{(p \times 1)}{\bar{\textbf{x}}}
    \underset{(1 \times p)}{\bm{\mu}^{\prime}}
    +
    n
    \underset{(p \times 1)}{\bar{\textbf{x}}}
    \underset{(1 \times p)}{\bm{\mu}^{\prime}}
    =
\]
\[
    =
    \underset{p \times p}{\textbf{0}}
\]
and
\[
    \sum_{j=1}^{n}{
        (\bar{\textbf{x}} - \bm{\mu})
        {(\textbf{x}_{j} - \bar{\textbf{x}})}^{\prime}
        }
    =
\]
\[
    =
    \sum_{j=1}^{n}{
        (\bar{\textbf{x}} - \bm{\mu})
        {(\textbf{x}_{j}^{\prime} - \bar{\textbf{x}}^{\prime})}
        }
    =
\]
\[
    =
    \sum_{i=1}^{n}{
        \left(
            \underset{(p \times 1)}{\bar{\textbf{x}}}
            \underset{(1 \times p)}{\textbf{x}_{j}^{\prime}}
            -
            \underset{(p \times 1)}{\bm{\mu}}
            \underset{(1 \times p)}{\textbf{x}_{j}^{\prime}}
            -
            \underset{(p \times 1)}{\bar{\textbf{x}}}
            \underset{(1 \times p)}{\bar{\textbf{x}}^{\prime}}
            +
            \underset{(p \times 1)}{\bm{\mu}}
            \underset{(1 \times p)}{\bar{\textbf{x}}^{\prime}}
        \right)
    }
    =
\]
\[
    =
    \sum_{i=1}^{n}{
        \left(
            \underset{(p \times 1)}{\bar{\textbf{x}}}
            \underset{(1 \times p)}{\textbf{x}_{j}^{\prime}}
        \right)
    }
    -
    \sum_{i=1}^{n}{
        \left(
            \underset{(p \times 1)}{\bm{\mu}}
            \underset{(1 \times p)}{\textbf{x}_{j}^{\prime}}
        \right)
    }
    -
    n
    \underset{(p \times 1)}{\bar{\textbf{x}}}
    \underset{(1 \times p)}{\bar{\textbf{x}}^{\prime}}
    +
    n
    \underset{(p \times 1)}{\bm{\mu}}
    \underset{(1 \times p)}{\bar{\textbf{x}}^{\prime}}
    =
\]
\[
    =
    n
    \underset{(p \times 1)}{\bar{\textbf{x}}}
    \underset{(1 \times p)}{\bar{\textbf{x}}^{\prime}}
    -
    n
    \underset{(p \times 1)}{\bm{\mu}}
    \underset{(1 \times p)}{\bar{\textbf{x}}^{\prime}}
    -
    n
    \underset{(p \times 1)}{\bar{\textbf{x}}}
    \underset{(1 \times p)}{\bar{\textbf{x}}^{\prime}}
    +
    n
    \underset{(p \times 1)}{\bm{\mu}}
    \underset{(1 \times p)}{\bar{\textbf{x}}^{\prime}}
    =
\]
\[
    =
    \underset{p \times p}{\textbf{0}}
\]
\underline{Long answer:}
\[
    \sum_{j=1}^{n}{
        (\textbf{x}_{j} - \bar{\textbf{x}})
        {(\bar{\textbf{x}} - \bm{\mu})}^{\prime}
    }
    =
\]
\[
    =
    \sum_{j=1}^{n}{
        \left(
            \begin{bNiceArray}{c}
                x_{j1} \\
                \vdots \\
                x_{jp}
            \end{bNiceArray}
            -
            \begin{bNiceArray}{c}
                \bar{x}_{1} \\
                \vdots \\
                \bar{x}_{p}
            \end{bNiceArray}
        \right)
        {\left(
            \begin{bNiceArray}{c}
                \bar{x}_{1} \\
                \vdots \\
                \bar{x}_{p}
            \end{bNiceArray}
            -
            \begin{bNiceArray}{c}
                \mu_{1} \\
                \vdots \\
                \mu_{p}
            \end{bNiceArray}
        \right)}^{\prime}
    }
    =
\]
\[
    =
    \sum_{j=1}^{n}{
        \left(
            \begin{bNiceArray}{c}
                x_{j1} - \bar{x}_{1} \\
                \vdots \\
                x_{jp} - \bar{x}_{p}
            \end{bNiceArray}
        \right)
        {\left(
            \begin{bNiceArray}{c}
                \bar{x}_{1} - \mu_{1} \\
                \vdots \\
                \bar{x}_{p} - \mu_{p}
            \end{bNiceArray}
        \right)}^{\prime}
    }
    =
\]
\[
    =
    \sum_{j=1}^{n}{
        \left(
            \begin{bNiceArray}{ccc}
                (x_{j1} - \bar{x}_{1}){(\bar{x}_{1} - \mu_{1})} &
                \cdots &
                (x_{j1} - \bar{x}_{1}){(\bar{x}_{p} - \mu_{p})} \\
                \vdots &
                \ddots &
                \vdots \\
                (x_{jp} - \bar{x}_{p}){(\bar{x}_{1} - \mu_{1})} &
                \cdots &
                (x_{jp} - \bar{x}_{p}){(\bar{x}_{p} - \mu_{p})}
            \end{bNiceArray}
        \right)
    }
    =
\]
{\small
\[
    =
    \sum_{j=1}^{n}{
        \left(
            \begin{bNiceArray}{ccc}
                (x_{j1}\bar{x}_{1} - \bar{x}_{1}\bar{x}_{1} - x_{j1}\mu_{1} + \bar{x}_{1}\mu_{1}) &
                \cdots &
                (x_{j1}\bar{x}_{p} - \bar{x}_{1}\bar{x}_{p}
                - x_{j1}\mu_{p} + \bar{x}_{1}\mu_{p}) \\
                \vdots &
                \ddots &
                \vdots \\
                (x_{jp}\bar{x}_{1} - \bar{x}_{p}\bar{x}_{1}
                - x_{jp}\mu_{1} + \bar{x}_{p}\mu_{1}) &
                \cdots &
                (x_{jp}\bar{x}_{p} - \bar{x}_{p}\bar{x}_{p}
                - x_{jp}\mu_{p} + \bar{x}_{p}\mu_{p})
            \end{bNiceArray}
        \right)
    }
    =
\]}
{\footnotesize
\[
    =
    \begin{bNiceArray}{ccc}
        \sum_{j=1}^{n}{(x_{j1}\bar{x}_{1} - \bar{x}_{1}\bar{x}_{1} - x_{j1}\mu_{1} + \bar{x}_{1}\mu_{1})} &
        \cdots &
        \sum_{j=1}^{n}{(x_{j1}\bar{x}_{p} - \bar{x}_{1}\bar{x}_{p}
        - x_{j1}\mu_{p} + \bar{x}_{1}\mu_{p})} \\
        \vdots &
        \ddots &
        \vdots \\
        \sum_{j=1}^{n}{(x_{jp}\bar{x}_{1} - \bar{x}_{p}\bar{x}_{1}
        - x_{jp}\mu_{1} + \bar{x}_{p}\mu_{1})} &
        \cdots &
        \sum_{j=1}^{n}{(x_{jp}\bar{x}_{p} - \bar{x}_{p}\bar{x}_{p}
        - x_{jp}\mu_{p} + \bar{x}_{p}\mu_{p})}
    \end{bNiceArray}
    =
\]}
{\tiny
\[
    =
    \begin{bNiceArray}{ccc}
        \sum_{j=1}^{n}{(x_{j1}\bar{x}_{1})} - n\bar{x}_{1}\bar{x}_{1} - \sum_{j=1}^{n}{(x_{j1}\mu_{1})} + n\bar{x}_{1}\mu_{1} &
        \cdots &
        \sum_{j=1}^{n}{(x_{j1}\bar{x}_{p})} - n\bar{x}_{1}\bar{x}_{p}
        - \sum_{j=1}^{n}{(x_{j1}\mu_{p})} + n\bar{x}_{1}\mu_{p} \\
        \vdots &
        \ddots &
        \vdots \\
        \sum_{j=1}^{n}{(x_{jp}\bar{x}_{1})} - n\bar{x}_{p}\bar{x}_{1}
        - \sum_{j=1}^{n}{(x_{jp}\mu_{1})} + n\bar{x}_{p}\mu_{1} &
        \cdots &
        \sum_{j=1}^{n}{(x_{jp}\bar{x}_{p})} - n\bar{x}_{p}\bar{x}_{p}
        - \sum_{j=1}^{n}{(x_{jp}\mu_{p})} + n\bar{x}_{p}\mu_{p}
    \end{bNiceArray}
    =
\]}
{\scriptsize
\[
    =
    \begin{bNiceArray}{ccc}
        n\bar{x}_{1}\bar{x}_{1} - n\bar{x}_{1}\bar{x}_{1} - n\bar{x}_{1}\mu_{1} + n\bar{x}_{1}\mu_{1} &
        \cdots &
        n\bar{x}_{1}\bar{x}_{p} - n\bar{x}_{1}\bar{x}_{p}
        - n\bar{x}_{1}\mu_{p} + n\bar{x}_{1}\mu_{p} \\
        \vdots &
        \ddots &
        \vdots \\
        n\bar{x}_{p}\bar{x}_{1} - n\bar{x}_{p}\bar{x}_{1}
        - n\bar{x}_{p}\mu_{1} + n\bar{x}_{p}\mu_{1} &
        \cdots &
        n\bar{x}_{p}\bar{x}_{p} - n\bar{x}_{p}\bar{x}_{p}
        - n\bar{x}_{p}\mu_{p} + n\bar{x}_{p}\mu_{p}
    \end{bNiceArray}
    =
\]}
\[
    =
    \begin{bNiceArray}{ccc}
        0 & \cdots & 0 \\
        \vdots & \ddots & \vdots \\
        0 & \cdots & 0
    \end{bNiceArray}
    =
    \underset{(p \times p)}{\textbf{0}}
\]
and
\[
    \sum_{j=1}^{n}{
        (\bar{\textbf{x}} - \bm{\mu})
        {(\textbf{x}_{j} - \bar{\textbf{x}})}^{\prime}
        }
    =
\]
\[
    =
    \sum_{j=1}^{n}{
        \left(
            \begin{bNiceArray}{c}
                \bar{x}_{1} \\
                \vdots \\
                \bar{x}_{p}
            \end{bNiceArray}
            -
            \begin{bNiceArray}{c}
                \mu_{1} \\
                \vdots \\
                \mu_{p}
            \end{bNiceArray}
        \right)
        {\left(
            \begin{bNiceArray}{c}
                x_{j1} \\
                \vdots \\
                x_{jp}
            \end{bNiceArray}
            -
            \begin{bNiceArray}{c}
                \bar{x}_{1} \\
                \vdots \\
                \bar{x}_{p}
            \end{bNiceArray}
        \right)}^{\prime}
    }
    =
\]
\[
    =
    \sum_{j=1}^{n}{
        \left(
            \begin{bNiceArray}{c}
                \bar{x}_{1} - \mu_{1} \\
                \vdots \\
                \bar{x}_{p} - \mu_{p}
            \end{bNiceArray}
        \right)
        {\left(
            \begin{bNiceArray}{c}
                x_{j1} - \bar{x}_{1} \\
                \vdots \\
                x_{jp} - \bar{x}_{p}
            \end{bNiceArray}
        \right)}^{\prime}
    }
    =
\]
\[
    =
    \sum_{j=1}^{n}{
        \left(
            \begin{bNiceArray}{ccc}
                (\bar{x}_{1} - \mu_{1})(x_{j1} - \bar{x}_{1}) &
                \cdots &
                (\bar{x}_{1} - \mu_{1})(x_{jp} - \bar{x}_{p}) \\
                \vdots &
                \ddots &
                \vdots \\
                (\bar{x}_{p} - \mu_{p})(x_{j1} - \bar{x}_{1}) &
                \cdots &
                (\bar{x}_{p} - \mu_{p})(x_{jp} - \bar{x}_{p})
            \end{bNiceArray}
        \right)
    }
    =
\]
{\small
\[
    =
    \sum_{j=1}^{n}{
        \left(
            \begin{bNiceArray}{ccc}
                (\bar{x}_{1}x_{j1} - \mu_{1}x_{j1}
                - \bar{x}_{1}\bar{x}_{1} + \mu_{1}\bar{x}_{1}) &
                \cdots &
                (\bar{x}_{1}x_{jp} - \mu_{1}x_{jp}
                - \bar{x}_{1}\bar{x}_{p} + \mu_{1}\bar{x}_{p}) \\
                \vdots &
                \ddots &
                \vdots \\
                (\bar{x}_{p}x_{j1} - \mu_{p}x_{j1}
                - \bar{x}_{p}\bar{x}_{1} - \mu_{p}\bar{x}_{1}) &
                \cdots &
                (\bar{x}_{p}x_{jp} - \mu_{p}x_{jp}
                - \bar{x}_{p}\bar{x}_{p} + \mu_{p}\bar{x}_{p})
            \end{bNiceArray}
        \right)
    }
    =
\]}
{\scriptsize
\[
    =
            \begin{bNiceArray}{ccc}
                \sum_{j=1}^{n}{(\bar{x}_{1}x_{j1} - \mu_{1}x_{j1}
                - \bar{x}_{1}\bar{x}_{1} + \mu_{1}\bar{x}_{1})} &
                \cdots &
                \sum_{j=1}^{n}{(\bar{x}_{1}x_{jp} - \mu_{1}x_{jp}
                - \bar{x}_{1}\bar{x}_{p} + \mu_{1}\bar{x}_{p})} \\
                \vdots &
                \ddots &
                \vdots \\
                \sum_{j=1}^{n}{(\bar{x}_{p}x_{j1} - \mu_{p}x_{j1}
                - \bar{x}_{p}\bar{x}_{1} - \mu_{p}\bar{x}_{1})} &
                \cdots &
                \sum_{j=1}^{n}{(\bar{x}_{p}x_{jp} - \mu_{p}x_{jp}
                - \bar{x}_{p}\bar{x}_{p} + \mu_{p}\bar{x}_{p})}
            \end{bNiceArray}
    =
\]}
{\tiny
\[
    =
    \begin{bNiceArray}{ccc}
        \sum_{j=1}^{n}{(\bar{x}_{1}x_{j1})} - \sum_{j=1}^{n}{(\mu_{1}x_{j1})}
        - n\bar{x}_{1}\bar{x}_{1} + n\mu_{1}\bar{x}_{1} &
        \cdots &
        \sum_{j=1}^{n}{(\bar{x}_{1}x_{jp})} - \sum_{j=1}^{n}{(\mu_{1}x_{jp})}
        - n\bar{x}_{1}\bar{x}_{p} + n\mu_{1}\bar{x}_{p} \\
        \vdots &
        \ddots &
        \vdots \\
        \sum_{j=1}^{n}{(\bar{x}_{p}x_{j1})} - \sum_{j=1}^{n}{(\mu_{p}x_{j1})}
        - n\bar{x}_{p}\bar{x}_{1} + n\mu_{p}\bar{x}_{1} &
        \cdots &
        \sum_{j=1}^{n}{(\bar{x}_{p}x_{jp})} - \sum_{j=1}^{n}{(\mu_{p}x_{jp})}
        - n\bar{x}_{p}\bar{x}_{p} + n\mu_{p}\bar{x}_{p}
    \end{bNiceArray}
    =
\]}
{\scriptsize
\[
    =
    \begin{bNiceArray}{ccc}
        n\bar{x}_{1}\bar{x}_{1} - n\mu_{1}\bar{x}_{1}
        - n\bar{x}_{1}\bar{x}_{1} + n\mu_{1}\bar{x}_{1} &
        \cdots &
        n\bar{x}_{1}\bar{x}_{p} - n\mu_{1}\bar{x}_{p}
        - n\bar{x}_{1}\bar{x}_{p} + n\mu_{1}\bar{x}_{p} \\
        \vdots &
        \ddots &
        \vdots \\
        n\bar{x}_{p}\bar{x}_{1} - n\mu_{p}\bar{x}_{1}
        - n\bar{x}_{p}\bar{x}_{1} + n\mu_{p}\bar{x}_{1} &
        \cdots &
        n\bar{x}_{p}\bar{x}_{p} - n\mu_{p}\bar{x}_{p}
        - n\bar{x}_{p}\bar{x}_{p} + n\mu_{p}\bar{x}_{p}
    \end{bNiceArray}
    =
\]}
\[
    =
    \begin{bNiceArray}{ccc}
        0 & \cdots & 0 \\
        \vdots & \ddots & \vdots \\
        0 & \cdots & 0
    \end{bNiceArray}
    =
    \underset{(p \times p)}{\textbf{0}}
\]