Given the data
\[
    {\large{\textbf{X}}}
    =
    \begin{bNiceArray}{ccc}
        3 & 6 & 0 \\
        4 & 4 & 3 \\
        \makebox[2em][c]{\textemdash} & 8 & 3 \\
        5 & \makebox[2em][c]{\textemdash} & \makebox[2em][c]{\textemdash}
    \end{bNiceArray}
\]
with missing components, use the prediction-estimation algorithm of Section 5.7 to
estimate $\bm{\mu}$, and $\bm{\Sigma}$. Determine the initial estimates, and iterate to find the first revised estimates.
\[
    \widetilde{\mu}_{1}
    =
    \frac{3+4+5}{3}
    =
    \frac{12}{3}
    =
    4
\]
\[
    \widetilde{\mu}_{2}
    =
    \frac{6+4+8}{3}
    =
    \frac{18}{3}
    =
    6
\]
\[
    \widetilde{\mu}_{3}
    =
    \frac{0+3+3}{3}
    =
    \frac{6}{3}
    =
    2
\]
\[
    \widetilde{\sigma}_{11}
    =
    \frac{
        {(3 - 4)}^{2}+
        {(4 - 4)}^{2}+
        {(4 - 4)}^{2}+
        {(5 - 4)}^{2}
    }{4}
    =
    \frac{1 + 1}{4}
    =
    \frac{1}{2}
\]
\[
    \widetilde{\sigma}_{22}
    =
    \frac{
        {(6 - 6)}^{2}+
        {(4 - 6)}^{2}+
        {(8 - 6)}^{2}+
        {(6 - 6)}^{2}
    }{4}
    =
    \frac{4 + 4}{4}
    =
    2
\]
\[
    \widetilde{\sigma}_{33}
    =
    \frac{
        {(0 - 2)}^{2}+
        {(3 - 2)}^{2}+
        {(3 - 2)}^{2}+
        {(2 - 2)}^{2}
    }{4}
    =
    \frac{4 + 1 + 1}{4}
    =
    \frac{3}{2}
\]

\[
    \widetilde{\sigma}_{12}
    =
    \frac{
        (3 - 4)(6 - 6)+
        (4 - 4)(4 - 6)+
        (4 - 4)(8 - 6)+
        (5 - 4)(6 - 6)+
    }{4}
    =
    0
\]
\[
    \widetilde{\sigma}_{13}
    =
    \frac{
        (3 - 4)(0 - 2)+
        (4 - 4)(3 - 2)+
        (4 - 4)(3 - 2)+
        (5 - 4)(2 - 2)+
    }{4}
    =
    \frac{1}{2}
\]
\[
    \widetilde{\sigma}_{23}
    =
    \frac{
        (6 - 6)(0 - 2)+
        (4 - 6)(3 - 2)+
        (8 - 6)(3 - 2)+
        (6 - 6)(2 - 2)+
    }{4}
    =
    0
\]

\underline{Observation 3, $\textbf{x}_{3}$:}
\newline
The first component of $\textbf{x}_{3}$ is missing, so we partition $\tilde{\bm{\mu}}$ and $\tilde{\bm{\Sigma}}$ as
\[
    \tilde{\bm{\mu}}
    =
    \begin{bNiceArray}{c}[margin]
        \widetilde{\mu}_{1} \\
        \widetilde{\mu}_{2} \\
        \widetilde{\mu}_{3} \\
        \CodeAfter \tikz \draw[dotted] (2-|1) -- (2-|last);
    \end{bNiceArray}
    =
    \begin{bNiceArray}{c}[margin]
        4 \\
        6 \\
        2 \\
        \CodeAfter \tikz \draw[dotted] (2-|1) -- (2-|last);
    \end{bNiceArray}
\]
\[
    \tilde{\bm{\Sigma}}
    =
    \begin{bNiceArray}{ccc}[margin]
        \widetilde{\sigma}_{11} & \widetilde{\sigma}_{12} & \widetilde{\sigma}_{13} \\
        \widetilde{\sigma}_{21} & \widetilde{\sigma}_{22} & \widetilde{\sigma}_{23} \\
        \widetilde{\sigma}_{31} & \widetilde{\sigma}_{32} & \widetilde{\sigma}_{33} \\
        \CodeAfter \tikz \draw[dotted] (2|-1) -- (2|-last);
        \CodeAfter \tikz \draw[dotted] (1|-2) -- (last|-2);
    \end{bNiceArray}
    =
    \begin{bNiceArray}{ccc}[margin]
        \frac{1}{2} & 0 & \frac{1}{2} \\
        0           & 2 & 0           \\
        \frac{1}{2} & 0 & \frac{3}{2} \\
        \CodeAfter \tikz \draw[dotted] (2|-1) -- (2|-last);
        \CodeAfter \tikz \draw[dotted] (1|-2) -- (last|-2);
    \end{bNiceArray}
    =
    \begin{bNiceArray}{cc}[margin]
        \widetilde{\bm{\Sigma}}_{11} & \widetilde{\bm{\Sigma}}_{12} \\
        \widetilde{\bm{\Sigma}}_{21} & \widetilde{\bm{\Sigma}}_{22} \\
        \CodeAfter \tikz \draw[dotted] (2-|1) -- (2-|last);
        \CodeAfter \tikz \draw[dotted] (1-|2) -- (last-|2);
    \end{bNiceArray}
\]
Using,
\[
    \widetilde{\textbf{x}}_{j}^{(1)} =
    E(\textbf{X}_{j}^{(1)}
      \big{\vert}
      \textbf{x}_{j}^{(2)};
      \widetilde{\bm{\mu}}, \widetilde{\bm{\Sigma}}
    )
    =
    \widetilde{\bm{\mu}}^{(1)}
    +
    \widetilde{\bm{\Sigma}}_{12}
    \widetilde{\bm{\Sigma}}_{22}^{-1}
    (\textbf{x}^{(2)} - \widetilde{\bm{\mu}}^{(2)})
    \Rightarrow
\]
\[
    \Rightarrow
    \widetilde{x}_{31}
    =
    \widetilde{\mu}_{1}
    +
    \widetilde{\bm{\Sigma}}_{12}
    \widetilde{\bm{\Sigma}}_{22}^{-1}
    \begin{bNiceArray}{r}
        x_{32} - \widetilde{\mu}_{2} \\
        x_{33} - \widetilde{\mu}_{3}
    \end{bNiceArray}
    =
\]
\[
    =
    4
    +
    \begin{bNiceArray}{rr}
        0 & \frac{1}{2}
    \end{bNiceArray}
    \left(\frac{1}{3}\right)
    \begin{bNiceArray}{rr}
        \frac{3}{2} & 0 \\
        0 & 2
    \end{bNiceArray}
    \begin{bNiceArray}{r}
        8 - 6 \\
        3 - 2
    \end{bNiceArray}
    =
\]
\[
    =
    4
    +
    \left(\frac{1}{3}\right)
    \begin{bNiceArray}{rr}
        0 & 1
    \end{bNiceArray}
    \begin{bNiceArray}{r}
        2 \\
        1
    \end{bNiceArray}
    =
    \frac{13}{3}
\]
The superscript $(1)$ is for missing values. The superscript $(2)$ is for observed values.

Computing the squared term,
\[
    \widetilde{
        \textbf{x}_{j}^{(1)}
        {\textbf{x}_{j}^{(1)}}^{\prime}
    }
    =
    E(\textbf{X}_{j}^{(1)}{\textbf{X}_{j}^{(1)}}^{\prime}
      \big{\vert}
      \tilde{\textbf{x}}_{j}^{(2)};
      \tilde{\bm{\mu}}, \tilde{\bm{\Sigma}}
    )
    =
    \widetilde{\bm{\Sigma}}_{11}
    -
    \tilde{\bm{\Sigma}}_{12}
    \tilde{\bm{\Sigma}}_{22}^{-1}
    \tilde{\bm{\Sigma}}_{21}
    +
    \widetilde{ \textbf{x} }_{j}^{(1)}
    \widetilde{ \textbf{x} }_{j}^{(1)\prime}
    \Rightarrow
\]
\[
    \Rightarrow
    \widetilde{x}_{31}^{2}
    =
    \widetilde{\sigma}_{11}
    -
    \tilde{\bm{\Sigma}}_{12}
    \tilde{\bm{\Sigma}}_{22}^{-1}
    \tilde{\bm{\Sigma}}_{21}
    +
    {\left(\widetilde{x}_{31}\right)}^{2}
    =
\]
\[
    =
    \frac{1}{2}
    -
    \begin{bNiceArray}{rr}
        0 & \frac{1}{2}
    \end{bNiceArray}
    \left(\frac{1}{3}\right)
    \begin{bNiceArray}{rr}
        \frac{3}{2} & 0 \\
        0 & 2
    \end{bNiceArray}
    \begin{bNiceArray}{r}
        0 \\
        \frac{1}{2}
    \end{bNiceArray}
    +
    {\left(\frac{13}{3}\right)}^{2}
    =
\]
\[
    \frac{1}{2}
    -
    \left(\frac{1}{3}\right)
    \begin{bNiceArray}{rr}
        0 & 1
    \end{bNiceArray}
    \begin{bNiceArray}{r}
        0 \\
        \frac{1}{2}
    \end{bNiceArray}
    +
    \frac{169}{9}
    =
    \frac{172}{9}
\]
Computing the cross-terms
\[
    \textbf{x}_{j}^{(1)}
    \textbf{x}_{j}^{(2)\prime}
    =
    E
    \left(
        \textbf{X}_{j}^{(1)}
        \textbf{X}_{j}^{(2)\prime}
        \big{\vert}
        \textbf{x}_{j}^{(2)\prime};
        \widetilde{\bm{\mu}},
        \widetilde{\bm{\Sigma}}
    \right)
    =
    \widetilde{\textbf{x}}_{j}^{(1)}
    \textbf{x}_{j}^{(2)\prime}
\]
\[
    \Rightarrow
    \widetilde{x_{31}}
        \begin{bNiceArray}{rr}
            x_{32}, & x_{33}
        \end{bNiceArray}
    =
    \widetilde{x_{31}}
    \begin{bNiceArray}{rr}
        x_{32}, & x_{33}
    \end{bNiceArray}
    =
    \frac{13}{3}
    \begin{bNiceArray}{rr}
        8, & 3
    \end{bNiceArray}
    =
    \begin{bNiceArray}{rr}
        \frac{104}{3}, & 13
    \end{bNiceArray}
\]

\underline{Observation 4, $\textbf{x}_{4}$:}
\newline
The second and third component of $\textbf{x}_{4}$ is missing, so we partition $\tilde{\bm{\mu}}$ and $\tilde{\bm{\Sigma}}$ as
\[
    \tilde{\bm{\mu}}
    =
    \begin{bNiceArray}{c}[margin]
        \widetilde{\mu}_{2} \\
        \widetilde{\mu}_{3} \\
        \widetilde{\mu}_{1} \\
        \CodeAfter \tikz \draw[dotted] (3-|1) -- (3-|last);
    \end{bNiceArray}
    =
    \begin{bNiceArray}{c}[margin]
        6 \\
        2 \\
        4 \\
        \CodeAfter \tikz \draw[dotted] (3-|1) -- (3-|last);
    \end{bNiceArray}
\]
 We moved $\widetilde{\mu}_{1}$ to the bottom.
\[
    \tilde{\bm{\Sigma}}
    =
    \begin{bNiceArray}{ccc}[margin]
        \widetilde{\sigma}_{22} & \widetilde{\sigma}_{23} & \widetilde{\sigma}_{21} \\
        \widetilde{\sigma}_{32} & \widetilde{\sigma}_{33} & \widetilde{\sigma}_{31} \\
        \widetilde{\sigma}_{12} & \widetilde{\sigma}_{13} & \widetilde{\sigma}_{11} \\
        \CodeAfter \tikz \draw[dotted] (3|-1) -- (3|-last);
        \CodeAfter \tikz \draw[dotted] (1|-3) -- (last|-3);
    \end{bNiceArray}
    =
    \begin{bNiceArray}{ccc}[margin]
        2 & 0           & 0 \\
        0 & \frac{3}{2} & \frac{1}{2}           \\
        0 & \frac{1}{2} & \frac{1}{2} \\
        \CodeAfter \tikz \draw[dotted] (3|-1) -- (3|-last);
        \CodeAfter \tikz \draw[dotted] (1|-3) -- (last|-3);
    \end{bNiceArray}
    =
    \begin{bNiceArray}{cc}[margin]
        \widetilde{\bm{\Sigma}}_{11} & \widetilde{\bm{\Sigma}}_{12} \\
        \widetilde{\bm{\Sigma}}_{21} & \widetilde{\bm{\Sigma}}_{22} \\
        \CodeAfter \tikz \draw[dotted] (2-|1) -- (2-|last);
        \CodeAfter \tikz \draw[dotted] (1-|2) -- (last-|2);
    \end{bNiceArray}
\]
We moved row 1 to the end and then moved column 1 to the end.
\newline
Using,
\[
    \widetilde{\textbf{x}}_{j}^{(1)} =
    E(\textbf{X}_{j}^{(1)}
      \big{\vert}
      \textbf{x}_{j}^{(2)};
      \widetilde{\bm{\mu}}, \widetilde{\bm{\Sigma}}
    )
    =
    \widetilde{\bm{\mu}}^{(1)}
    +
    \widetilde{\bm{\Sigma}}_{12}
    \widetilde{\bm{\Sigma}}_{22}^{-1}
    (\textbf{x}^{(2)} - \widetilde{\bm{\mu}}^{(2)})
    \Rightarrow
\]
\[
    \Rightarrow
    \begin{bNiceArray}{c}
        \widetilde{x}_{42} \\
        \widetilde{x}_{43}
    \end{bNiceArray}
    =
    \begin{bNiceArray}{c}
        \widetilde{\mu}_{2} \\
        \widetilde{\mu}_{3}
    \end{bNiceArray}
    +
    \widetilde{\bm{\Sigma}}_{12}
    \widetilde{\bm{\Sigma}}_{22}^{-1}
    (x_{41} - \widetilde{\mu}_{1})
    =
\]
\[
    =
    \begin{bNiceArray}{c}
        6 \\
        2
    \end{bNiceArray}
    +
    \begin{bNiceArray}{r}
        0 \\
        \frac{1}{2}
    \end{bNiceArray}
    \left(2\right)
    (5 - 4)
    =
\]
\[
    =
    \begin{bNiceArray}{c}
        6 \\
        2
    \end{bNiceArray}
    +
    \begin{bNiceArray}{c}
        0 \\
        1
    \end{bNiceArray}
    =
    \begin{bNiceArray}{r}
        6 \\
        3
    \end{bNiceArray}
\]
The superscript $(1)$ is for missing values. The superscript $(2)$ is for observed values.

Computing the squared term,
\[
    \widetilde{
        \textbf{x}_{j}^{(1)}
        {\textbf{x}_{j}^{(1)}}^{\prime}
    }
    =
    E(\textbf{X}_{j}^{(1)}{\textbf{X}_{j}^{(1)}}^{\prime}
      \big{\vert}
      \tilde{\textbf{x}}_{j}^{(2)};
      \tilde{\bm{\mu}}, \tilde{\bm{\Sigma}}
    )
    =
    \widetilde{\bm{\Sigma}}_{11}
    -
    \tilde{\bm{\Sigma}}_{12}
    \tilde{\bm{\Sigma}}_{22}^{-1}
    \tilde{\bm{\Sigma}}_{21}
    +
    \widetilde{ \textbf{x} }_{j}^{(1)}
    \widetilde{ \textbf{x} }_{j}^{(1)\prime}
    \Rightarrow
\]
\[
    \Rightarrow
    \begin{bNiceArray}{cc}
        \widetilde{x_{42}^{2}}   & \widetilde{x_{42}x_{43}} \\
        \widetilde{x_{43}x_{42}} & \widetilde{x_{43}^{2}}
    \end{bNiceArray}
    =
    \widetilde{\Sigma}_{11}
    -
    \tilde{\bm{\Sigma}}_{12}
    \left(\frac{1}{\widetilde{\sigma}_{11}}\right)
    \tilde{\bm{\Sigma}}_{21}
    +
    \begin{bNiceArray}{c}
        \widetilde{x}_{42} \\
        \widetilde{x}_{43}
    \end{bNiceArray}
    \begin{bNiceArray}{cc}
        \widetilde{x}_{42} & \widetilde{x}_{43}
    \end{bNiceArray}
    =
\]
\[
    =
    \begin{bNiceArray}{cc}
        2 & 0           \\
        0 & \frac{3}{2}
    \end{bNiceArray}
    -
    \begin{bNiceArray}{c}
        0 \\
        \frac{1}{2}
    \end{bNiceArray}
    \left(\frac{1}{(1/2)}\right)
    \begin{bNiceArray}{cc}
        0 & \frac{1}{2}
    \end{bNiceArray}
    +
    \begin{bNiceArray}{c}
        6 \\
        3
    \end{bNiceArray}
    \begin{bNiceArray}{cc}
        6 & 3
    \end{bNiceArray}
    =
\]
\[
    =
    \begin{bNiceArray}{cc}
        2 & 0           \\
        0 & \frac{3}{2}
    \end{bNiceArray}
    -
    \begin{bNiceArray}{cc}
        0 & 0           \\
        0 & \frac{1}{2}
    \end{bNiceArray}
    +
    \begin{bNiceArray}{cc}
        36 & 18 \\
        18 & 9
    \end{bNiceArray}
    =
    \begin{bNiceArray}{cc}
        38 & 18 \\
        18 & 10
    \end{bNiceArray}
\]
Computing the cross-terms
\[
    \textbf{x}_{j}^{(1)}
    \textbf{x}_{j}^{(2)\prime}
    =
    E
    \left(
        \textbf{X}_{j}^{(1)}
        \textbf{X}_{j}^{(2)\prime}
        \big{\vert}
        \textbf{x}_{j}^{(2)\prime};
        \widetilde{\bm{\mu}},
        \widetilde{\bm{\Sigma}}
    \right)
    =
    \widetilde{\textbf{x}}_{j}^{(1)}
    \textbf{x}_{j}^{(2)\prime}
\]
\[
    \begin{bNiceArray}{c}
        \widetilde{x}_{42} \\
        \widetilde{x}_{43}
    \end{bNiceArray}
    x_{41}
    =
    \begin{bNiceArray}{c}
        \widetilde{x}_{42}x_{41} \\
        \widetilde{x}_{43}x_{41}
    \end{bNiceArray}
    =
    \begin{bNiceArray}{c}
        6(5) \\
        3(5)
    \end{bNiceArray}
    =
    \begin{bNiceArray}{c}
        30 \\
        15
    \end{bNiceArray}
\]

Computing
\[
    \widetilde{\textbf{T}}_{1}
    =
    \sum_{j=1}^{n}{\textbf{X}_{j}}
    =
    \begin{bNiceArray}{c}
        x_{11} \\
        x_{12} \\
        x_{13}
    \end{bNiceArray}
    +
    \begin{bNiceArray}{c}
        x_{21} \\
        x_{22} \\
        x_{23}
    \end{bNiceArray}
    +
    \begin{bNiceArray}{c}
        \widetilde{x}_{31} \\
        x_{32} \\
        x_{33}
    \end{bNiceArray}
    +
    \begin{bNiceArray}{c}
        x_{41} \\
        \widetilde{x}_{42} \\
        \widetilde{x}_{43}
    \end{bNiceArray}
    =
\]
\[
    =
    \begin{bNiceArray}{c}
        3 \\
        6 \\
        0
    \end{bNiceArray}
    +
    \begin{bNiceArray}{c}
        4 \\
        4 \\
        3
    \end{bNiceArray}
    +
    \begin{bNiceArray}{c}
        13/3 \\
        8 \\
        3
    \end{bNiceArray}
    +
    \begin{bNiceArray}{c}
        5 \\
        6 \\
        3
    \end{bNiceArray}
    =
    \begin{bNiceArray}{c}
        49/3 \\
        24 \\
        9
    \end{bNiceArray}
\]
\[
    \widetilde{\textbf{T}}_{2}
    =
    \sum_{j=1}^{n}{
        \textbf{X}_{j}
        \textbf{X}_{j}^{\prime}
        }
    =
    \sum_{j=1}^{4}
    \begin{bNiceArray}{c}
        x_{j1} \\
        x_{j2} \\
        x_{j3}
    \end{bNiceArray}
    \begin{bNiceArray}{ccc}
        x_{j1} & x_{j2} & x_{j3}
    \end{bNiceArray}
    =
\]
\[
    =
    \sum_{j=1}^{4}
    \begin{bNiceArray}{ccc}
        x_{j1}^{2} & x_{j1}x_{j2} & x_{j1}x_{j3} \\
        x_{j2}x_{j1} & x_{j2}^{2} & x_{j2}x_{j3} \\
        x_{j3}x_{j1} & x_{j3}x_{j2} & x_{j3}^{2}
    \end{bNiceArray}
    =
\]
\begin{multline*}
    =
    \begin{bNiceArray}{ccc}
        x_{11}^{2} & x_{11}x_{12} & x_{11}x_{13} \\
        x_{12}x_{11} & x_{12}^{2} & x_{12}x_{13} \\
        x_{13}x_{11} & x_{13}x_{12} & x_{13}^{2}
    \end{bNiceArray} \\
    +
    \begin{bNiceArray}{ccc}
        x_{21}^{2} & x_{21}x_{22} & x_{21}x_{23} \\
        x_{22}x_{21} & x_{22}^{2} & x_{22}x_{23} \\
        x_{23}x_{21} & x_{23}x_{22} & x_{23}^{2}
    \end{bNiceArray} \\
    +
    \begin{bNiceArray}{ccc}
        \widetilde{x}_{31}^{2} & \widetilde{x}_{31}x_{32} & \widetilde{x}_{31}x_{33} \\
        x_{32}\widetilde{x}_{31} & x_{32}x_{32} & x_{32}x_{33} \\
        x_{33}\widetilde{x}_{31} & x_{33}x_{32} & x_{33}x_{33}
    \end{bNiceArray} \\
    +
    \begin{bNiceArray}{ccc}
        x_{41}x_{41} & x_{41}\widetilde{x}_{42} & x_{41}\widetilde{x}_{43} \\
        \widetilde{x}_{42}x_{41} & \widetilde{x}_{42}^{2} & \widetilde{x}_{42}\widetilde{x}_{43} \\
        \widetilde{x}_{43}x_{41} & \widetilde{x}_{43}\widetilde{x}_{42} & \widetilde{x}_{43}^{2}
    \end{bNiceArray}
    =
\end{multline*}
    \begin{align*}
        \scriptstyle \text{Component 11} &= \scriptstyle  x_{11}^{2} + x_{21}^{2} + \widetilde{x}_{31}^{2} + x_{41}^{2} = {(3)}^{2} + {(4)}^{2} + \left(\frac{172}{9}\right) + {(3)}^{2} = \frac{622}{9} \\
        \scriptstyle \text{Component 22} &= \scriptstyle  x_{12}^{2} + x_{22}^{2} + x_{32}^{2} + \widetilde{x}_{42}^{2} = {(6)}^{2} + {(4)}^{2} + {(8)}^{2} + 38 = 154 \\
        \scriptstyle  \text{Component 33} &= \scriptstyle  x_{13}^{2} + x_{23}^{2} + x_{33}^{2} + \widetilde{x}_{43}^{2} = {(0)}^{2} + {(3)}^{2} + {(3)}^{2} + 10 = 28 \\
        \scriptstyle  \text{Component 21} &= \scriptstyle  x_{12}x_{11} + x_{22}x_{21} + x_{32}\widetilde{x}_{31} + \widetilde{x}_{42}x_{41} = (6)(3) + (4)(4) + \frac{104}{3} + 30 = \frac{296}{3} \\
        \scriptstyle  \text{Component 31} &= \scriptstyle  x_{13}x_{11} + x_{23}x_{21} + x_{33}\widetilde{x}_{31} + \widetilde{x}_{43}x_{41} = (0)(3) + (3)(4) + 13 + 15 = 40 \\
        \scriptstyle  \text{Component 32} &= \scriptstyle  x_{13}x_{12} + x_{23}x_{22} + x_{33}x_{32} + \widetilde{x}_{43}\widetilde{x}_{42} = (0)(6) + (3)(4) + (3)(8) + 18 = 54
    \end{align*}

so we have

\[
    \widetilde{\textbf{T}}_{2}
    =
    \begin{bNiceArray}{ccc}
        \frac{622}{9} & \frac{296}{3} & 40 \\
        \frac{296}{3} & 154           & 54 \\
        40            & 54            & 28
    \end{bNiceArray}
\]
Computing $\widetilde{\bm{\mu}}$ and $\widetilde{\bm{\Sigma}}$,
\[
    \tilde{\bm{\mu}}
    =
    \frac{1}{4}
    \widetilde{\textbf{T}}_{1}
    =
    \frac{1}{4}
    \begin{bNiceArray}{c}
        \frac{49}{3} \\
        24 \\
        9
    \end{bNiceArray}
    =
    \begin{bNiceArray}{c}
        4.0833 \\
        6.0000 \\
        2.2500
    \end{bNiceArray}
\]

\[
    \tilde{\bm{\Sigma}}
    =
    \frac{1}{n}
    \widetilde{\textbf{T}}_{2}
    +
    \widetilde{\bm{\mu}}
    \widetilde{\bm{\mu}}^{\prime}
    =
    \frac{1}{4}
    \begin{bNiceArray}{ccc}
        \frac{622}{9} & \frac{296}{3} & 40 \\
        \frac{296}{3} & 154           & 54 \\
        40            & 54            & 28
    \end{bNiceArray}
    -
    \begin{bNiceArray}{c}
        \frac{49}{3} \\
        24 \\
        9
    \end{bNiceArray}
    \begin{bNiceArray}{ccc}
        \frac{49}{3} & 24 & 9
    \end{bNiceArray}
    =
\]
\[
    =
    \begin{bNiceArray}{ccc}
        \frac{622}{36} & \frac{296}{12} & 10           \\
        \frac{296}{12} & \frac{154}{4}  & \frac{54}{4} \\
        10             & \frac{54}{4}   & \frac{28}{4}
    \end{bNiceArray}
    -
    \begin{bNiceArray}{ccc}
        \frac{2401}{144} & \frac{3528}{144} & \frac{1323}{144} \\
        \frac{3528}{144} & \frac{5184}{144} & \frac{1944}{144} \\
        \frac{1323}{144} & \frac{1944}{144} & \frac{729}{144}
    \end{bNiceArray}
    =
\]
\[
    =
    \frac{1}{144}
    \begin{bNiceArray}{ccc}
        87  & 24  & 117 \\
        24  & 360 & 0   \\
        117 & 0   & 279
    \end{bNiceArray}
    =
    \begin{bNiceArray}{ccc}
        0.6042 & 0.1667 & 0.8125 \\
        0.1667 & 2.5000 & 0.0000 \\
        0.8125 & 0.0000 & 1.9375  
    \end{bNiceArray}
\]